\documentclass{article}
\usepackage{amsmath}
\usepackage{fullpage}
%\usepackage{graphicx}
\usepackage{tikz}
% \allowdisplaybreaks
\usepackage[aux]{rerunfilecheck}

\newcommand{\ds}{\displaystyle}

\input{../common.tex}

\title{\commonPSTitleZeroTwoFour\ Solutions}
\author{\commonAuthor}
\date{\commonDateZeroTwoFour}

\begin{document}
\maketitle
\begin{enumerate}
\item %1
  \begin{enumerate}
  \item %1a
    We apply the sum rule for derivatives:
    \begin{align*}
      f'(x) &= \frac{d}{dx} (2x^3 + \cos x)
      \\
            &= \frac{d}{dx} 2x^3 + \frac{d}{dx} \cos x
      \\
            &= 2 \frac{d}{dx} x^3 + \frac{d}{dx} \cos x
      \\
            &= 2 \cdot 3 x^2 - \sin x
      \\
            &= 6 x^2 - \sin x
    \end{align*}
    using the constant multiple rule, power rule, and rule for $\cos
    x$. 
  \item %1b
    Using the product rule,
    \begin{align*}
      G'(t) &= \frac{d}{dt} (t^2 \cos t)
      \\
            &= \left(\frac{d}{dt} t^2\right) \cos t
              + t^2 \frac{d}{dt} \cos t
      \\
            &= 2t \cos t + t^2 (-\sin t)
      \\
            &= 2t \cos t - t^2 \sin t
    \end{align*}
    where we used the power rule and the rule for $\cos t$ on the
    second line.
% \item %1c
  \item %1d
    By the quotient rule
    \begin{align*}
      \frac{d}{d\theta} \frac{1-\sin\theta}{\tan\theta+\cos\theta}
      &= \frac{(\tan\theta+\cos\theta)(-\cos\theta) -
        (1-\sin\theta)(\sec^2\theta-\sin\theta)}{
        (\tan\theta+\cos\theta)^2}
    \end{align*}
    You can do lots of algebra and apply various trig identities to
    simplify the expression slightly, but my advice is to leave it
    alone, unless you need to do something else with it that requires
    simplification.
  \end{enumerate}
\item %2
  To find a tangent line we need to find its slope, which is a derivative.
  \begin{align*}
    y' &= \frac{d}{dx} x \cos x
    \\
       &= \frac{dx}{dx} \cos x + x \frac{d}{dx} \cos x
    \\
       &= \cos x + x (-\sin x)
    \\
       &= \cos x - x \sin x
  \end{align*}
  where we applied the product rule.  We evaluate the derivative at
  the base point $x=\pi$ to find the slope:
  \begin{equation*}
    y'(\pi) = \cos\pi - \pi \sin \pi = -1 - \pi (0) = -1
  \end{equation*}
  So the equation of the tangent line is
  \begin{equation*}
    y - (-\pi) = -1 (x - \pi)
    \implies y + \pi = \pi - x
    \implies y = -x
  \end{equation*}
  The negative reciprocal of $-1$ is $-1/-1 = 1$, which is the slope
  of the normal line, so the equation of the normal line is
  \begin{equation*}
    y - (-\pi) = 1 (x -\pi)
    \implies
    y + \pi = x -\pi
    \implies
    y = x - 2\pi
  \end{equation*}
  % EJD Show graph
\item %3
  We calculated the first derivative in the previous problem.  We take
  the derivative of that to obtain the second derivative:
  \begin{align*}
    \frac{d^2y}{dx^2} &= \frac{d}{dx} \frac{dy}{dx}
    \\
                      &= \frac{d}{dx} (\cos x - x \sin x)
    \\
                      &= \frac{d}{dx} \cos x - \frac{d}{dx} x\sin x
    \\
                      &= -\sin x - \sin x - x \cos x
    \\
                      &= -2\sin x - x \cos x
  \end{align*}
\item %4
  The function has a horizontal tangent where its derivative is $0$.
  So we need to calculate the derivative:
  \begin{equation*}
    f'(x) = 1 - \sin x
  \end{equation*}
  We need to solve the equation
  \begin{equation*}
    f'(x) = 0 \implies 1 - \sin x = 0 \implies \sin x = 1
  \end{equation*}
  The $\sin^{-1}$ button on the calculator can give one solution: $x =
  \sin^{-1} (1) = \pi/2$.  You should look at a graph of $\sin x$ to
  find all the other solutions: $x = \pi/2 \pm 2k\pi$,
  $k=0,1,2,\ldots$.
  % EJD: include graph
\item %5
  \begin{enumerate}
  \item %5a
    Multiply the numerator and denominator by $2$ to obtain
    \begin{equation*}
      \lim_{x\to 0} \frac{\sin 2x}{x}
      = \lim_{x\to 0} 2\frac{\sin 2x}{2x}
      = 2
    \end{equation*}
  \item %5b
    Multiply the numerator and denominator by $2x$, and then by $3x$, to
    obtain
    \begin{equation*}
      \lim_{x\to 0} \frac{\sin 2x}{\sin 3x}
      = \lim_{x\to 0} \frac{\sin 2x}{2x} \cdot \frac{2x}{3x} \cdot
      \frac{3x}{\sin 3x}
      = 1 \cdot \frac{2}{3} \cdot 1 = \frac{2}{3}
    \end{equation*}
  \item %5c
    Call the limit in the question $L$.
    By the product rule for limits we have
    \begin{equation*}
      L = \lim_{t\to 0} \left( \frac{\sin 2t}{t} \right)^3
      = \left( \lim_{t\to 0} \frac{\sin 2t}{t} \right)^3
    \end{equation*}
    provided the limit inside the bracket exists.  But it is just a variation
    on the basic trig limit we studied:
    \begin{equation*}
      \lim_{t\to 0} \frac{\sin 2t}{t}
      = \lim_{t\to 0} 2 \frac{\sin 2t}{2t}
      = 2 \lim_{t\to 0} \frac{\sin 2t}{2t}
      = 2 \cdot 1 = 2
    \end{equation*}
    Putting it all together, $L=2^3=8$.
  \item %5d
    \textbf{Solution 1:} Call the limit $L$.  Write $\tan\theta$ in
    terms of $\sin\theta$ and $\cos\theta$:
    \begin{equation*}
      L
      = \lim_{\theta\to 0} \frac{\cos\theta - 1}{\tan\theta}
      = \lim_{\theta\to 0} \frac{\cos\theta -
        1}{\frac{\sin\theta}{\cos\theta}}
      = \lim_{\theta\to 0} \frac{(\cos\theta-1)\cos\theta}{
        \sin\theta} 
    \end{equation*}
    Divide both numerator and denominator by $\theta$:
    \begin{equation*}
      L = \lim_{\theta\to 0} \frac{\frac{\cos\theta-1}{\theta}
        \cos\theta}{
        \frac{\sin\theta}{\theta}}
    \end{equation*}
    By the quotient rule for limits we have 
    \begin{equation*}
      L = \frac{\lim_{\theta\to 0}\frac{\cos\theta -
          1}{\theta}\lim_{\theta\to 0} \cos\theta}{
        \lim_{\theta\to 0}\frac{\sin\theta}{\theta}}
      = \frac{0 \cdot 1}{1} = 0
    \end{equation*}

    \textbf{Solution 2:}  Multiply numerator and denominator by the
    ``conjugate'' $\cos\theta+1$ to obtain
    \begin{equation*}
      L = \lim_{\theta\to 0} \frac{\cos\theta - 1}{\sin\theta}
      = \lim_{\theta\to 0} \frac{\cos\theta - 1}{\tan\theta} 
      \cdot \frac{\cos\theta+1}{\cos\theta+1}
      = \lim_{\theta\to 0} \frac{\cos^2\theta - 1}{\tan\theta(\cos\theta+1)} 
    \end{equation*}
    Using the Pythagorean identity $\sin^2\theta+\cos^2\theta=1$,
    \begin{align*}
      L &= \lim_{\theta\to 0} \frac{\cos^2\theta - 1}{\tan\theta(\cos\theta+1)} 
          = \lim_{\theta\to 0}
          \frac{-\sin^2\theta}{(\sin\theta/\cos\theta)(\cos\theta+1)}
      \\
        &= \lim_{\theta\to 0} \frac{-\sin\theta}{(\cos\theta+1)/\cos\theta}
        = \frac{-\sin 0}{(\cos 0+1)/\cos 0} = \frac{-0}{(1+1)/1} =
        \frac{0}{2}
      \\
        &= 0
    \end{align*}
  \end{enumerate}
\item %6
  This is a question from the lecture.  Using the definition of $\sec$
  in terms of $\cos$ and the quotient rule,
  \begin{align*}
    \frac{d}{dx} \sec x &= \frac{d}{dx} \frac{1}{\cos x}
    \\
                        &= \frac{\cos x (0) - 1 (-\sin x)}{\cos^2 x}
    \\
                        &=\frac{\sin x}{\cos^2 x}
    \\
                        &=\frac{1}{\cos x} \cdot \frac{\sin x}{\cos x}
    \\
                        &=\sec x \tan x
  \end{align*}
\item %7
  This is a question from the lecture.  The solution is essentially
  parallel to the calculation of the derivative for $\sin$.  Using the
  definition of derivative,
  \begin{align*}
    \frac{d}{dx} \cos x &= \lim_{h\to 0} \frac{\cos(x+h) - \cos x}{h}
  \end{align*}
  Now we need an angle addition formula for $\cos$, which you can look
  up in the trig identity tables in the textbook:
  \begin{align*}
    \cos(x+h) = \cos x \cos h - \sin x \sin h
  \end{align*}
  Continuing with our calculation,
  \begin{align*}
    \frac{d}{dx} \cos x &= \lim_{h\to 0}
                          \frac{\cos x \cos h -\sin x \sin h -\cos x}{
                          h}
    \\
                        &= \cos x \lim_{h\to 0} \frac{\cos h-1}{h}
                          - \sin x\lim_{h\to 0} \frac {\sin h}{h}
    \\
                        &= \cos x (0) - \sin x (1)
    \\
                        &= -\sin x
  \end{align*}
  by the basic trig limits.
\item %8
  \begin{enumerate}
  \item %8a
    Note that $\mu$ and $W$ are constants in this problem, so we treat
    them as constants when we apply the differentiation rules.  By the
    quotient rule,
    \begin{align*}
      \frac{dF}{d\theta} &= \frac{(\mu\sin\theta+\cos\theta)(0) - \mu
                           W(\mu\cos\theta - \sin\theta)}{
                           (\mu\sin\theta+\cos\theta)^2}
      \\
                         &= -\frac{\mu W(\mu\cos\theta-\sin\theta)}{
                           (\mu\sin\theta+\cos\theta)^2}
    \end{align*}
  \item %8b
    By the previous, $dF/d\theta=0$ implies that
    \begin{equation*}
      \mu\cos\theta-\sin\theta = 0
    \end{equation*}
    (Note: we are assuming that $\mu$ and $W$ are not $0$.  What
    happens if either number is $0$?  What would that mean
    physically?)

    To solve that equation, we move $\sin\theta$ to the right-hand
    side and then divide by $\cos\theta$:
    \begin{align*}
      \mu\cos\theta &= \sin\theta \\
      \mu &= \frac{\sin\theta}{\cos\theta} \\
      \mu &= \tan\theta
    \end{align*}
    You can solve that equation with a calculator using the
    $\tan^{-1}$ button: $\theta= \tan^{-1} \mu$ gives the solution as
    an angle in radians if your calculator is set to radian mode, or
    in degrees if your calculator is set to degree mode.  For example,
    if $\mu=1$ your calculator should give the answer $\pi/4$ radians,
    or $45^\circ$.
  \end{enumerate}
% \item %9
%   You should try taking several derivatives and looking for patterns.
%   However, there is a trick you could use to help speed up the process.
%   Consider the functions
%   \begin{align*}
%     f(x) &= x\sin x + x\cos x + a\sin x + b\cos x \\
%     g(x) &= x\sin x - x\cos x + c\sin x + d\cos x
%   \end{align*}
%   By the constant multiple, sum, and product rules we have
%   \begin{equation*}
%     Df(x) = a \cos x + ax(-\sin x) + b\sin x + bx\cos x - c\sin x + d\cos x
%     = bx\cos x - a x\sin x + (a+d) \cos x + (b-c)\sin x
% \item %10
\end{enumerate}
\end{document}

%% Some leftover junk??
  %   \textbf{Solution 1:}  Write
  %   \begin{equation*}
  %     \lim_{\theta\to 0} \frac{\cos\theta - 1}{\tan\theta}
  %     = \lim_{\theta\to 0} \frac{\frac{\cos\theta - 1}{\theta}}{
  %       \frac{\sin\theta}{\theta}\cdot\cos\theta}
  %   \end{equation*}
  %   By the quotient rule for limits we have 
  %   \begin{equation*}
  %     \lim_{\theta\to 0} \frac{\frac{\cos\theta - 1}{\theta}}{
  %       \frac{\sin\theta}{\theta}}
  %     = \frac{\lim_{\theta\to 0} \frac{\cos\theta - 1}{\theta}}{
  %       \lim_{\theta\to 0} \frac{\sin\theta}{\theta}}
  %   \end{equation*}
  %   provided both limits exist and the limit in the denominator is not $0$.
  %   But both limits do exist: they are the basic trig limits; the numerator
  %   is $0$ and the denominator is $1$, so the original limit exists and
  %   equals $0$.

  %   \textbf{Solution 2:}  Multiply numerator and denominator by the
  %   ``conjugate'' $\cos\theta+1$ to obtain
  %   \begin{equation*}
  %     \lim_{\theta\to 0} \frac{\cos\theta - 1}{\sin\theta}
  %     = \lim_{\theta\to 0} \frac{\cos\theta - 1}{\sin\theta} 
  %     \cdot \frac{\cos\theta+1}{\cos\theta+1}
  %     = \lim_{\theta\to 0} \frac{\cos^2\theta - 1}{\sin\theta(\cos\theta+1)} 
  %   \end{equation*}
  %   Using the Pythagorean identity $\sin^2\theta+\cos^2\theta=1$,
  %   \begin{equation*}
  %     \lim_{\theta\to 0} \frac{\cos^2\theta - 1}{\sin\theta(\cos\theta+1)} 
  %     = \lim_{\theta\to 0} \frac{-\sin^2\theta}{\sin\theta(\cos\theta+1)}
  %     = \lim_{\theta\to 0} \frac{-\sin\theta}{\cos\theta+1}
  %     = \frac{-\sin 0}{\cos 0+1} = 0
  %   \end{equation*}
  % \item %1b
  %   Call the limit in the question $L$.
  %   By the chain rule for limits (or the product rule for limits), we have
  %   \begin{equation*}
  %     L = \lim_{t\to 0} \left( \frac{\sin 3t}{t} \right)^2
  %     = \left( \lim_{t\to 0} \frac{\sin 3t}{t} \right)^2
  %   \end{equation*}
  %   provided the limit inside the bracket exists.  But it is just a variation
  %   on the basic trig limit we studied:
  %   \begin{equation*}
  %     \lim_{t\to 0} \frac{\sin 3t}{t}
  %     = \lim_{t\to 0} 3 \frac{\sin 3t}{3t}
  %     = 3 \lim_{t\to 0} \frac{\sin 3t}{3t}
  %     = 3 \cdot 1
  %   \end{equation*}
  %   Putting it all together, $L=9$.
  % \item %1c
  %   Multiply numerator and denominator by $x$ to obtain
  %   \begin{equation*}
  %     \lim_{x\to 0} \frac{\sin(x^2)}{x}
  %     = \lim_{x\to 0} \frac{\sin(x^2)}{x^2} \cdot x
  %     = \lim_{x\to 0} \frac{\sin(x^2)}{x^2} \cdot \lim_{x\to 0} x
  %     = 1 \cdot 0 = 0
  %   \end{equation*}
