%\documentclass{article}
%\usepackage{beamerarticle}
\documentclass[serif,ignorenonframetext]{beamer}

\input{../common.tex}

\usepackage{mathptmx}
\usepackage{multirow}

\newcommand{\ds}{\displaystyle}

\mode<article>{}
\mode<presentation>{\usetheme{\commonTheme}\usecolortheme{\commonColorTheme}}

\title{\commonTitleZeroTwoSix}
\subtitle{\commonSubtitleZeroTwoSix}
\author{\commonAuthor}
\institute{\commonInstitute}
\date{\commonDateZeroTwoSix}


\begin{document}


%\section*{Outline}

\begin{frame}
  \titlepage
\end{frame}

\begin{frame}
  \frametitle{Contents}
  \tableofcontents
\end{frame}



\section{Implicit Differentiation}

\subsection{Implicit Functions}

\begin{frame}
  \frametitle{Implicit and Explicit Functions}
  \begin{columns}
  \column{0.65\textwidth}
  \begin{itemize}[<+->]
  \item Consider the curve defined by $x^2+y^2=1$.
  \item That expression can be solved for $y$ to get
    two different continuous functions.
  \item $y=\sqrt{1-x^2}$
  \item $y=-\sqrt{1-x^2}$
  \item We say that $y=\sqrt{1-x^2}$ and $y=-\sqrt{1-x^2}$
    are \textbf{explicit} functions.
  \item The formula $x^2+y^2=1$ is an \textbf{implicit}
    definition of those functions.
  \end{itemize}
  \column{0.35\textwidth}
  \only<1-2>{\includegraphics[width=\textwidth]{cont0.eps}}%
  \only<3>{\includegraphics[width=\textwidth]{cont0a.eps}}%
  \only<4-5>{\includegraphics[width=\textwidth]{cont0b.eps}}%
  \only<6>{\includegraphics[width=\textwidth]{cont0.eps}}%
  \end{columns}
\end{frame}

\begin{frame}
  \frametitle{Explicit Functions are Hard to Find}
  \begin{columns}
  \column{0.65\textwidth}
  \begin{itemize}[<+->]
  \item Consider the curve defined by $x^3+y^3=6xy$.
  \item That expression can be solved for $y$ only with
    considerable difficulty.
  \item For example, the simplest explicit function
    determine by $x^3+y^3=6xy$ is
    \begin{align*}
      y =& \sqrt[3]{-\frac{1}{2}x^3+\sqrt{\frac{1}{4}x^6-8x^3}} \\
         &+ \sqrt[3]{-\frac{1}{2}x^3-\sqrt{\frac{1}{4}x^6-8x^3}}
    \end{align*}
  \end{itemize}
  \column{0.35\textwidth}
  \only<1-2>{\includegraphics[width=\textwidth]{cont1.eps}}%
  \only<3->{\includegraphics[width=\textwidth]{cont1a.eps}}%
  \end{columns}
\end{frame}

\subsection{Implicit Differentiation}

\begin{frame}
  \frametitle{Implicit Differentiation}
  \begin{itemize}[<+->]
  \item Some implicit functions can't be solved explicitly at all.
  \item But we may need to differentiate them anyway.
  \item We use the process of implicit differentiation.
  \item We differentiate an expression as if it were a function,
    where we use the chain rule every time we see a $y$.
  \item For example, for $\ds x^2+y^2 = 1$ we have
    \begin{align*}
      \uncover<+->{\frac{d}{dx} (x^2+y^2) = \frac{d}{dx} 1}%
      \uncover<+->{&\implies \frac{d}{dx} x^2 + \frac{d}{dx} y^2 = 0 \\}%
      \uncover<+->{&\implies 2x + 2y \frac{dy}{dx} = 0 \\}%
      \uncover<+->{&\implies \frac{dy}{dx} = -\frac{x}{y}}%
    \end{align*}
  \end{itemize}
\end{frame}

\begin{frame}
  \frametitle{Comparing Implicit and Explicit Differentiation}
  \begin{itemize}[<+->]
  \item Note that in the result of implicit differentiation we have a $y$.
  \item We usually can't get rid of the $y$ unless the function can be
    expressed in explicit form $y=f(x)$.
  \item The two ways of calculating the derivative should agree.  
    Recall the example $x^2+y^2=1$.
  \item Differentiating implicitly then substituting 
    $y=\sqrt{1-x^2}$, we have 
    $\ds\frac{dy}{dx} = -\frac{x}{y} = -\frac{x}{\sqrt{1-x^2}}$.
  \item On the other hand, starting with $y=\sqrt{1-x^2}$ 
    we have 
    \begin{align*}
      \frac{dy}{dx} 
      \uncover{&= \frac{d}{dx} (1-x^2)^{1/2} \\}%
      \uncover{&= \frac{1}{2} (1-x^2)^{-1/2} \frac{d}{dx} (1-x^2) }%
      \uncover{= -\frac{x}{\sqrt{1-x^2}}}%
    \end{align*}
  \item The two methods agree.  (What happens if $y=-\sqrt{1-x^2}$?)
  \end{itemize}
\end{frame}

\begin{frame}
  \frametitle{Implicit Differentiation is the Better Option}
  \begin{itemize}[<+->]
  \item In most cases, it is difficult or impossible to put an implicit
    function in explicit form.  Consider $x^3+y^3=6xy$.
  \item The explicit form for $y$ is too difficult for us to remember.
  \item The only good option is implicit differentiation:
    \begin{align*}
      \uncover<+->{\frac{d}{dx} (x^3+y^3)= \frac{d}{dx} (6xy) }%
      \uncover<+->{&\implies \frac{d}{dx} x^3 + \frac{d}{dx} y^3 
      = 6\left(\frac{d}{dx} x\right) y + 6 x \frac{d}{dx} y \\}%
      \uncover<+->{&\implies 3x^2 + 3y^2 \frac{dy}{dx} 
      = 6y + 6x \frac{dy}{dx} \\}%
      \uncover<+->{&\implies (3y^2-6x) \frac{dy}{dx} = 6y-3x^2 \\}%
      \uncover<+->{&\implies \frac{dy}{dx} = \frac{6y-3x^2}{3y^2-6x}}%
    \end{align*}
  \item Note that to complete the calculation I had to solve for $dy/dx$.
  \end{itemize}
\end{frame}

\begin{frame}
  \frametitle{When Implicit Differentiation is Necessary}
  \begin{itemize}[<+->]
  \item Sometimes it is impossible to put an implicit function in
    explicit form.  Consider $\sin(xy)=x^2+y$.
    I can't solve for $y$ explicitly.
  \item We have no choice but to use implicit differentiation.
    \begin{align*}
      \uncover<+->{\frac{d}{dx} \sin (xy) = \frac{d}{dx} (x^2 + y)}%
      \uncover<+->{&\implies \cos(xy) \frac{d}{dx} (xy) 
        = \frac{d}{dx} x^2 + \frac{d}{dx}y \\}%
      \uncover<+->{&\implies \cos(xy) (y+xy') = 2x + y' \\}%
      \uncover<+->{&\implies (x\cos(xy) - 1) y' = 2x - y\cos(xy) \\}%
      \uncover<+->{&\implies y' = \frac{2x-y\cos(xy)}{x\cos(xy)-1}}%
    \end{align*}
  \item We can now construct tangents on the curve, \emph{if we know a point
    on the curve}.  Points on the curve will be given, or special $x$ values
    where $y$ can be solved explicitly will be chosen, or points on the curve
    can be approximated by numerical methods.
  \end{itemize}
\end{frame}

\begin{frame}
  \frametitle{Second Derivatives by Implicit Differentiation}
  \begin{itemize}[<+->]
  \item We can also find second derivatives by implicit differentiation.
    Again consider $x^2+y^2=1$.
  \item By implicit differentiation we have the first derivative is
    $\ds y' = -\frac{x}{y}$.
  \item Differentiating a second time by the quotient rule we have
    \begin{align*}
      y'' = \frac{-y+xy'}{y^2}
    \end{align*}
  \item Substituting $y'=-x/y$ we have
    \begin{align*}
      y'' = \frac{-y+x(-x/y)}{y^2} 
      \uncover<+->{= -\frac{y^2+x^2}{y^3}}%
      \uncover<+->{= -\frac{1}{y^3}}%
    \end{align*}
  \item Compare that with finding the second derivative of the explicit
    function.
  \end{itemize}
\end{frame}


\subsection{Examples and Exercises}

\begin{frame}
  \frametitle{Examples}
  \begin{enumerate}
  \item Find $y'$ where $x\tan y = y-1$.
  \item Find $y''$ if $x^6+y^6=1$.
  \item Find the equations of the tangent line and normal line
    to the curve $x^2+4xy+y^2=13$ at the point $(2,1)$.
  \item Find the points on the ellipse $x^2+2y^2=1$ where the
    tangent line has slope $1$.
  \item Show that the length of the portion of any tangent
    line to the astroid $x^{2/3} + y^{2/3} = a^{2/3}$ cut off by
    the coordinate axes is constant.
  \end{enumerate} 
\end{frame}

\begin{frame}
  \frametitle{Exercises}
  Now you should work on Problem Set~2.6.  After you have finished it,
  you should try the following additional exercises from Section~2.6:
  \begin{itemize}
  \item[2.6] 
    C-level: 1--4, 5--20, 25--30, 31--32, 33--34, 35--38, 39--40; \\ 
    B-level: 43, 44--45, 46--47; \\
    A-level: 48, 49--52, 53--54, 55, 57--62
  \end{itemize}
\end{frame}


\end{document}

