%%% MATH110-PS021-Solutions.tex --- 
%% 
%% Filename: MATH110-PS021-Solutions.tex
%% Description: 
%% Author: U-ORONYA\edwar
%% Maintainer: 
%% Created: Sun Jan 29 21:34:17 2023 (-0600)
%% Version: 
%% Package-Requires: ()
%% Last-Updated: Sun Jan 29 23:34:38 2023 (-0600)
%%           By: U-ORONYA\edwar
%%     Update #: 39
%% URL: 
%% Doc URL: 
%% Keywords: 
%% Compatibility: 
%% 
%%%%%%%%%%%%%%%%%%%%%%%%%%%%%%%%%%%%%%%%%%%%%%%%%%%%%%%%%%%%%%%%%%%%%%
%% 
%%% Commentary: 
%% 
%% 
%% 
%%%%%%%%%%%%%%%%%%%%%%%%%%%%%%%%%%%%%%%%%%%%%%%%%%%%%%%%%%%%%%%%%%%%%%
%% 
%%% Change Log:
%% 
%% 
%%%%%%%%%%%%%%%%%%%%%%%%%%%%%%%%%%%%%%%%%%%%%%%%%%%%%%%%%%%%%%%%%%%%%%
%%
%% Copyright (C) 2023 Edward Doolittle
%% 
%%%%%%%%%%%%%%%%%%%%%%%%%%%%%%%%%%%%%%%%%%%%%%%%%%%%%%%%%%%%%%%%%%%%%%
%% 
%%% Code:


\documentclass{article}
\usepackage{amsmath}
\usepackage{fullpage}
%\usepackage{graphicx}
\usepackage{tikz,pgfplots}
\pgfplotsset{compat=1.13}
% \allowdisplaybreaks
\usepackage[aux]{rerunfilecheck}

\newcommand{\ds}{\displaystyle}

\input{../common.tex}

\title{\commonPSTitleZeroTwoOne\ Solutions}
\author{\commonAuthor}
\date{\commonDateZeroTwoOne}


\begin{document}
\maketitle
\begin{enumerate}
\item %1
  Recall that the derivative from first principles is
  \begin{equation*}
    f'(x) = \lim_{h\to 0} \frac{f(x+h)-f(x)}{h}
  \end{equation*}
  To evaluate the above expression, we first evaluate $f(x+h)$,
  simplifying if possible, then evaluate the limit.
  \begin{enumerate}
  \item %1a
    We have
    \begin{align*}
      f(x+h) &= (x+h)^2 - 2(x+h) - 3
               = x^2 + 2xh + h^2 - 2x - 2h - 3
      \\
      f(x+h) - f(x) &= x^2 + 2xh + h^2 - 2x - 2h - 3 - x^2 + 2x + 3
                      = 2xh + h^2 - 2h
    \end{align*}
    Then
    \begin{align*}
      f'(x) &= \lim_{h\to 0} \frac{f(x+h)-f(x)}{h}
      \\
      &= \lim_{h\to 0} \frac{2xh + h^2 - 2h}{h}
      \\
      &= \lim_{h\to 0} (2x + h - 2)
      \\
      &= 2x - 2
    \end{align*}
    At the point $(0,-3)$ we have $x=0$ so $f'(0) = 2(0)-2 = -2$,
    which is the slope of the tangent line at $x=0$.
  \item %1b
    We use the point-slope form for the equation of the tangent line.
    The point slope form is
    \begin{equation*}
      y - y_0 = m(x-x_0)
    \end{equation*}
    where $(x_0,y_0)$ is the point and $m$ is the slope.  In our case,
    $(x_0,y_0)=(0,-3)$ and $m=-2$ from the previous answer, so the
    tangent line has equation
    \begin{equation*}
      y - (-3) = (-2) (x-0) \implies y + 3 = -2x \implies y = -2x - 3
    \end{equation*}
  \item %1c
    See Figure~\ref{fig:graphParabola}.
    \begin{figure}[htbp]
      \centering
      \begin{tikzpicture}
        \draw[gray,very thin] (-1,-5) grid (2,1);
        \draw[->] (-1,0)--(2,0);
        \draw[->] (0,-5)--(0,1);
        \draw[color=red, line width = 0.50mm]   plot[smooth,domain=-1:2]
        (\x, {-3-2*\x+(\x)^2});
        \draw[color=blue, line width = 0.50mm]
        plot[smooth,domain=-1:1] (\x, {-3-2*\x});
        \node[label={45:{(0,-3)}},circle,fill,inner sep=2pt] at (0,-3) {};
      \end{tikzpicture}
      \caption{Graphs of $y=x^2-2x-3$ and $y=-2x-3$}
      \label{fig:graphParabola}
    \end{figure}
  \end{enumerate}
\item %2
  \begin{enumerate}
  \item %2a
    We have
    \begin{align*}
      f(x+h) &= \frac{1}{x+h+1} \\
      f(x) &= \frac{1}{x+1} \\
      f(x+h)-f(x) &= \frac{1}{x+h+1} - \frac{1}{x+1} = \frac{(x+1) -
        (x+h+1)}{(x+h+1)(x+1)}
      = \frac{-h}{(x+h+1)(x+1)} \\
      \frac{f(x+h) - f(x)}{h} &= \frac{-1}{(x+h+1)(x+1)} \\
      f'(x) &= \lim_{h\to 0} \frac{f(x+h)-f(x)}{h} = \lim_{h\to 0}
      \frac{-1}{(x+h+1)(x+1)} = \frac{-1}{(x+1)^2}
    \end{align*}
    Substituting $x=0$,
    \begin{equation*}
      f'(0) = \frac{-1}{(0+1)^2} = -1
    \end{equation*}
    Using point-slope form, the equation of the tangent line is
    \begin{equation*}
      y - y_0 = m(x-x_0) \implies y - 1 = (-1) (x-0) \implies y - 1 =
      -x \implies y = -x + 1
    \end{equation*}
  \item %2b
    We have
    \begin{align*}
      f(x+h) &= \sqrt{2(x+h)-1} \\
      f(x) &= \sqrt{2x-1} \\
      f(x+h) - f(x) &= \sqrt{2(x+h)-1} - \sqrt{2x-1} \\
      \frac{f(x+h) - f(x)}{h} &= \frac{\sqrt{2(x+h)-1} -
        \sqrt{2x-1}}{h} \\
      f'(x) &= \lim_{h\to 0} \frac{f(x+h) - f(x)}{h} = \lim_{h\to 0}
      \frac{\sqrt{2(x+h)-1} - \sqrt{2x-1}}{h}
    \end{align*}
    To evaluate limits like this, multiply by the conjugate radical:
    \begin{align*}
      f'(x) &= \lim_{h\to 0} \frac{\sqrt{2x+2h-1} - \sqrt{2x-1}}{h}
              \times \frac{\sqrt{2x+2h-1} + \sqrt{2x-1}}{\sqrt{2x+2h-1} +
              \sqrt{2x-1}}
      \\
            &= \lim_{h\to 0} \frac{(2x+2h-1) -
              (2x-1)}{h(\sqrt{2x+2h-1}-\sqrt{2x-1})}
      \\
            &= \lim_{h\to 0} \frac{2h}{h(\sqrt{2x+2h-1}-\sqrt{2x-1})}
      \\
            &= \frac{2}{\sqrt{2x-1}+\sqrt{2x-1}} = \frac{2}{2\sqrt{2x-1}}
      \\
            &= \frac{1}{\sqrt{2x-1}}
    \end{align*}
    Substituting $x=5$ gives $f'(5) = 1/(2(5)-1) = 1/9$.  The equation
    of the tangent line is $y-3 = 1/9(x-5)$, which can be rearranged
    to $y=(1/9) x - 22/9$.
  \item %2c
    We have
    \begin{align*}
      f(x+h) &= (x+h)^3 - 4(x+h) = x^3 + 3x^2 h + 3xh^2 + h^3 - 4x -
      4h \\
      f(x) &= x^3 - 4x \\
      f(x+h) - f(x) &= 3x^2 h + 3xh^2 + h^3 - 4h \\
      \frac{f(x+h) - f(x)}{h} &= \frac{3x^2h + 3xh^2 - h^3 - 4h}{h} =
      3x^2 + 3xh - h^2 - 4 \\
      f'(x) &= \lim_{h\to 0} \frac{f(x+h)-f(x)}{h} = \lim_{h\to 0}
      3x^2 + 3xh - h^2 - 4 = 3x^2 - 4
    \end{align*}
    At $x=-1$, $f'(-1) = 3(-1)^2 - 4 = 3 -4 = -1$.  The equation of
    the tangent line is $y-3 = (-1)(x-(-1))$ or $y-3 = -x -1$ or
    $y=-x+2$.
  \item %2d
    We have
    \begin{align*}
      f(x+h) &= \frac{(x+h)^2}{2(x+h)-1} = \frac{x^2+2xh+h^2}{2x+2h-1}
      \\
      f(x) &= \frac{x^2}{2x-1} \\
      f(x+h) - f(x) &= \frac{x^2+2xh+h^2}{2x+2h-1} - \frac{x^2}{2x-1}
                      = \frac{(x^2+2xh+h^2)(2x-1)-(2x+2h-1)x^2}{(2x+2h-1)(2x-1)}
                      \\
                      &= \frac{2x^3 - x^2 + 4x^2h - 2xh + 2xh^2 - h^2 - 2x^3 - 2x^2h +
                        x^2 }{(2x+2h-1)(2x-1)} 
                        = \frac{4x^2h-2xh-h^2}{(2x+2h-1)(2x-1)} \\
      \frac{f(x+h) - f(x)}{h} &= \frac{4x^2h-2xh-h^2}{(2x+2h-1)(2x-1)}
                                = \frac{4x^2 - 2x -h}{(2x+2h+1)(2x-1)} \\
      f'(x) &= \lim_{h\to 0} \frac{4x^2 - 2x - h}{(2x+2h-1)(2x-1)}
      = \frac{4x^2 - 2x}{(2x-1)(2x-1)} = \frac{4x^2-2x}{(2x-1)^2}
    \end{align*}
  \end{enumerate}
\item %3
  \begin{enumerate}
  \item We have
    \begin{align*}
      f(a+h) &= 10 + 3(a+h)^2 - (a+h)^3 = 10 + 3a^2 + 6ah + 3h^2
               - a^3 - 3a^2h - 3ah^2 - h^3 \\
      f(a) &= 10 + 3a^2 - a^3 \\
      f(a+h)-f(a) &= 10 + 3a^2 + 6ah + 3h^2
                    - a^3 - 3a^2h - 3ah^2 - h^3 - 10 - 3a^2 + a^3 \\
             &= 6ah + 3h^2 - 3a^2h - 3ah^2 - h^3 \\
      \frac{f(a+h)-f(a)}{h} &= \frac{6ah+3h^2-3a^2h-3ah^2-h^3}{h}
    \end{align*}
    Taking the limit,
    \begin{align*}
      f'(a) &= \lim_{h\to 0} \frac{f(a+h)-f(a)}{h} \\
            &= \lim_{h\to 0} \frac{6ah+3h^2-3a^2h-3ah^2-h^3}{h} \\
            &= \lim_{h\to 0} (6a + 3h - 3a^2 - 3ah - h^2) \\
            &= 6a - 3a^2
    \end{align*}
  \item Now that we have a formula for the slope of the tangent line,
    we can apply it to obtain the slope immediately in both cases.  In
    the first case,
    \begin{displaymath}
      m = f'(1) = 6(1) - 3(1)^2 = 6 - 3 = 3
    \end{displaymath}
    so the point-slope form of the tangent line is
    \begin{displaymath}
      y - 12 = 3(x-1)
    \end{displaymath}
    You can further simplify your answer but that is not necessary.
    In the second case,
    \begin{displaymath}
      m = f'(3) = 6(3) - 3(3)^2 = 18 - 27 = -9
    \end{displaymath}
    so the point-slope form of the tangent line is
    \begin{displaymath}
      y - 10 = -9(x-3)
    \end{displaymath}
  \item See Figure~\ref{fig:graphCubic}.
    \begin{figure}[htbp]
      \centering
      \begin{tikzpicture}
        \draw[gray,very thin] (0,0) grid (4,15);
        \draw[->] (0,0)--(4,0);
        \draw[->] (0,0)--(0,15);
        \draw[color=red, line width = 0.50mm]   plot[smooth,domain=0:3.723]
        (\x, {10+3*(\x)^2-(\x)^3});
        \draw[color=blue, line width = 0.50mm]
        plot[smooth,domain=0:2] (\x, {3*\x+9});
        \draw[color=blue, line width = 0.50mm]
        plot[smooth,domain=2.4444:4] (\x, {-9*\x+37});
        \node[label={20:{(1,12)}},circle,fill,inner sep=2pt] at (1,12) {};
        \node[label={160:{(3,10)}},circle,fill,inner sep=2pt] at (3,10) {};
      \end{tikzpicture}
      \caption{Graphs of $y=10+3x^2-x^3$ and $y=3x+9$ and $y=-9x+37$}
      \label{fig:graphCubic}
    \end{figure}
  \end{enumerate}
\item %4
  Instantaneous velocity is the derivative.  Since we need the
  velocity at several moments $t=1$, $t=2$, and $t=3$, we should find
  a general formula for the derivative.  We have
  \begin{align*}
    f(a+h) &= \frac{1}{a+h} \\
    f(a) &= \frac{1}{a} \\
    f(a+h)-f(a) &= \frac{1}{a+h} - \frac{1}{a} = \frac{a - a - h}{(a+h)(a)}
                  = \frac{-h}{(a+h)(a)} \\
    \frac{f(a+h)-f(a)}{h} &= \frac{-h}{(a+h)(a)(h)}
  \end{align*}
  Taking the limit,
  \begin{align*}
    v(a) = s'(a) &= \lim_{h\to 0} \frac{f(a+h)-f(a)}{h} \\
    &= \lim_{h\to 0} \frac{-h}{(a+h)(a)(h)} \\
    &= \lim_{h\to 0} \frac{-1}{(a+h)(a)} \\
    &= \frac{-1}{(a)(a)} \\
    &= \frac{-1}{a^2}
  \end{align*}
  Then at times $a=1$, $a=2$, and $a=3$ we have
  \begin{align*}
    v(1) &= \frac{-1}{1^2} = -1 \\
    v(2) &= \frac{-1}{2^2} = -\frac{1}{4} \\
    v(3) &= \frac{-1}{3^2} = -\frac{1}{9}
  \end{align*}
  where all velocity units are m/s.  Finally, the speeds are the
  absolute values of the velocities, so the speeds are
  \begin{align*}
    |v(a)| &= \left| -\frac{1}{a^2} \right| = \frac{1}{a^2} \\
    |v(1)| &= |-1| = 1 \\
    |v(2)| &= \left| -\frac{1}{4} \right| = \frac{1}{4} \\
    |v(3)| &= \left| -\frac{1}{9} \right| = \frac{1}{9}
  \end{align*}
  again in m/s.  Note that in $|v(a)|$ it is potentially tricky to get
  the sign right in general, but the fraction $1/a^2$ is always
  positive.
\item %5
  Note that there are many possible answers to this question.  First,
  we place a dot on an empty grid representing the point $(0,1)$
  through which the graph passes, and we draw a small line segment
  with slope $-1$ passing through the point $(0,1)$ representing the
  tangent line to the graph at the point.  See
  Figure~\ref{fig:four-conditions-1}(a).  Next, we draw a line segment
  of slope $0$ at a point $(1,y_1)$.  We are not given a condition on
  $y_1$ so we pick any $y_1$ (we should pick a value less than $1$ to
  get a nice graph).  See Figure~\ref{fig:four-conditions-1}(b).  We
  do the same thing with a small line segment of slope $3$ at the
  point $(2,y_2)$, where $y_2$ can be anything (but we should pick a
  value greater than $y_1$ to get a nice graph).  See
  Figure~\ref{fig:four-conditions-2}(c).  Finally, we sketch a nice
  smooth graph passing through the three points we have drawn, which
  is tangent to the three line segments we have drawn.  See
  Figure~\ref{fig:four-conditions-2}(d).
  \begin{figure}[htbp]
    \centering
    $\begin{array}{c@{\hspace{0.5in}}c}
    \begin{tikzpicture}[scale=1]
      \draw[gray,very thin] (-1,0) grid (4,7);
      \draw[->] (-1,0)--(4,0);
      \draw[->] (0,0)--(0,7);
      %\draw[color=red,domain=-1:3,samples=200] plot(\x,{(\x)^3/3-\x+1});
      \draw[color=black,domain=-0.5:0.5] plot(\x,{-\x+1});
      \fill[color=black] (0,1) circle (0.05);
      %\draw[color=black,domain=0.5:1.5] plot(\x,{1/3});
      %\fill[color=black] (1,1/3) circle (0.05);
      %\draw[color=black,domain=1.75:2.25] plot(\x,{3*(\x-2)+5/3});
      %\fill[color=black] (2,5/3) circle (0.05);
    \end{tikzpicture}
    &
    \begin{tikzpicture}[scale=1]
      \draw[gray,very thin] (-1,0) grid (4,7);
      \draw[->] (-1,0)--(4,0);
      \draw[->] (0,0)--(0,7);
      %\draw[color=red,domain=-1:3,samples=200] plot(\x,{(\x)^3/3-\x+1});
      \draw[color=black,domain=-0.5:0.5] plot(\x,{-\x+1});
      \fill[color=black] (0,1) circle (0.05);
      \draw[color=black,domain=0.5:1.5] plot(\x,{1/3});
      \fill[color=black] (1,1/3) circle (0.05);
      %\draw[color=black,domain=1.75:2.25] plot(\x,{3*(\x-2)+5/3});
      %\fill[color=black] (2,5/3) circle (0.05);
    \end{tikzpicture}
    \\
    \mbox{(a) Conditions $f(0)=1$, $f'(0)=-1$}
    &
    \mbox{(b) Adding condition $f'(1)=0$}
    \end{array}$
    \caption{First two conditions for graph}
    \label{fig:four-conditions-1}
  \end{figure}
  \begin{figure}[htbp]
    \centering
    $\begin{array}{c@{\hspace{0.5in}}c}
    \begin{tikzpicture}[scale=1]
      \draw[gray,very thin] (-1,0) grid (4,7);
      \draw[->] (-1,0)--(4,0);
      \draw[->] (0,0)--(0,7);
      %\draw[color=red,domain=-1:3,samples=200] plot(\x,{(\x)^3/3-\x+1});
      \draw[color=black,domain=-0.5:0.5] plot(\x,{-\x+1});
      \fill[color=black] (0,1) circle (0.05);
      \draw[color=black,domain=0.5:1.5] plot(\x,{1/3});
      \fill[color=black] (1,1/3) circle (0.05);
      \draw[color=black,domain=1.75:2.25] plot(\x,{3*(\x-2)+5/3});
      \fill[color=black] (2,5/3) circle (0.05);
    \end{tikzpicture}
    &
    \begin{tikzpicture}[scale=1]
      \draw[gray,very thin] (-1,0) grid (4,7);
      \draw[->] (-1,0)--(4,0);
      \draw[->] (0,0)--(0,7);
      \draw[color=red,domain=-1:3,samples=200] plot(\x,{(\x)^3/3-\x+1});
      \draw[color=black,domain=-0.5:0.5] plot(\x,{-\x+1});
      \fill[color=black] (0,1) circle (0.05);
      \draw[color=black,domain=0.5:1.5] plot(\x,{1/3});
      \fill[color=black] (1,1/3) circle (0.05);
      \draw[color=black,domain=1.75:2.25] plot(\x,{3*(\x-2)+5/3});
      \fill[color=black] (2,5/3) circle (0.05);
    \end{tikzpicture}
    \\
    \mbox{(c) Adding Condition $f'(2)=3$}
    &
    \mbox{(d) Graph Consistent with (c)}
    \end{array}$
    \caption{Third Condition, and Graph Consistent with Conditions}
    \label{fig:four-conditions-2}
  \end{figure}
\item %6
  \begin{enumerate}
  \item We have
    \begin{align*}
      f(a+h) &= 4(a+h)^2 - (a+h)^3
               = 4a^2 + 8ah + 4h^2 - a^3 - 3a^2h - 3ah^2 - h^3 \\
      f(a) &= 4a^2 - a^3 \\
      f(a+h)-f(a) &= 4a^2 + 8ah + 4h^2 - a^3 - 3a^2 h - 3ah^2 - h^3 - 4a^2 + a^3
      \\
             &= 8ah + 4h^2 - 3a^2 h - 3ah^2 - h^3
    \end{align*}
    Taking limits of the difference quotient,
    \begin{align*}
      f'(a) &= \lim_{h\to 0} \frac{8ah+4h^2-3a^2h-3ah^2-h^3}{h} \\
            &= \lim_{h\to 0} (8a + 4h - 3a^2 - 3ah - h^2) \\
            &= 8a - 3a^2
    \end{align*}
  \item By the binomial theorem we have
    \begin{align*}
      f(a+h) &= (a+h)^4 - 5(a+h) = a^4 + 4a^3h+6a^2h^2+4ah^3+h^4-5a-5h \\
      f(a) &= a^4 - 5a \\
      f(a+h)-f(a) &= a^4 + 4a^3h + 6a^2h^2 + 4ah^3 + h^4 - 5a - 5h - a^4 + 5a \\
             &=4a^3h + 6a^2h^2 + 4ah^3 + h^4 - 5h
    \end{align*}
    Taking the limit of the difference quotient,
    \begin{align*}
      f'(a) &= \lim_{h\to 0} \frac{4a^3h + 6a^2h^2 + 4ah^3 + h^4 - 5h}{h} \\
            &= \lim_{h\to 0} (4a^3 + 6a^2 h + 4ah^2 + h^3 - 5) \\
            &= 4a^3 - 5
    \end{align*}
  \item We have
    \begin{align*}
      f(a+h) &= \frac{(a+h)^2 + 1}{a+h-2} = \frac{a^2+2ah+h^2+1}{a+h-2} \\
      f(a) &= \frac{a^2+1}{a-2} \\
      f(a+h)-f(a) &= \frac{a^2+2ah+h^2+1}{a+h-2} - \frac{a^2+1}{a-2} \\
             &= \frac{(a^2+2ah+h^2+1)(a-2)-(a^2+1)(a+h-2)}{(a+h-2)(a-2)} \\
             &= \frac{a^3 + 2a^2h + ah^2 + a - 2a^2-4ah-2h^2-2
               - a^3 - a^2h + 2a^2 - h + 2}{(a+h-2)(a-2)} \\
             &= \frac{a^2h + ah^2 - 4ah - 2h^2 - h}{(a+h-2)(a-2)}
    \end{align*}
    Taking the limit of the difference quotient,
    \begin{align*}
      f'(a) &= \lim_{h\to 0} \frac{a^2h+ah^2-4ah-2h^2-h}{h(a+h-2)(a-2)} \\
            &= \lim_{h\to 0} \frac{a^2 + ah - 4a - 2h - 1}{(a+h-2)(a-2)} \\
            &= \frac{a^2 - 4a - 1}{(a-2)^2}
    \end{align*}
  \item We have
    \begin{align*}
      f(a+h) &= \sqrt{3a + 3h + 1} \\
      f(a) &= \sqrt{3a+1} \\
      f(a+h)-f(a) &= \sqrt{3a + 3h + 1} - \sqrt{3a + 1}
    \end{align*}
    Taking the limit of the difference quotient and evaluating the
    limit by multiplying by the conjugate radical,
    \begin{align*}
      f'(a) &= \lim_{h\to 0} \frac{\sqrt{3a+3h+1}-\sqrt{3a+1}}{h} \\
            &= \lim_{h\to 0} \frac{\sqrt{3a+3h+1}-\sqrt{3a+1}}{h}
       \times \frac{\sqrt{3a+3h+1}+\sqrt{3a+1}}{\sqrt{3a+3h+1}+\sqrt{3a+1}} \\
     &= \lim_{h\to 0} \frac{(3a+3h+1)-(3a+1)}{h(\sqrt{3a+3h+1}+\sqrt{3a+1})} \\
            &= \lim_{h\to 0} \frac{3h}{h(\sqrt{3a+3h+1}+\sqrt{3a+1})} \\
            &= \lim_{h\to 0} \frac{3}{\sqrt{3a+3h+1}+\sqrt{3a+1}} \\
            &= \frac{3}{2\sqrt{3a+1}}
    \end{align*}
  \end{enumerate}
\item %7
  We have
  \begin{align*}
    y(t+h) &= 5(t+h) - 4.9(t+h)^2 = 5t + 5h - 4.9t^2 - 9.8 th - 4.9
             h^2 \\
    y(t) &= 5t - 4.9 t^2 \\
    y(t+h) - y(t) &= 5h - 9.8 th - 4.9 h^2 \\
    \frac{y(t+y)-y(t)}{h} &= 5 - 9.8 t - 4.9 h \\
    y' &= \lim_{h\to 0} \frac{y(t+h)-y(t)}{h} = \lim_{h\to 0}
         (5-9.8t-4.9h) = 5-9.8t
  \end{align*}
  At $t=0.5$ seconds, $y'(0.5) = 5-9.8(0.5) = 5-4.9 = 0.1$ meters per
  second.  Positive velocities are upward (and negative velocities
  would be downward) in this problem.
\item %8
  We have to figure out how to represent some of the numbers in the
  expressions differently.
  \begin{enumerate}
  \item Write $32=2^5$.  Then we have $f(x)=x^5$ and $a=2$.  Check.
  \item Write $4=\sqrt{16}$.  Then we have $f(x)=\sqrt{x}$ and
    $a=16$.  Check.
  %\item Write $1=e^0$.  Then we have $f(x)=e^x$ and $a=0$.  Check.
  \item Note that $\ds \sin \frac{\pi}{2} = 1$ so we can write the
    expression as
    \begin{displaymath}
      \lim_{t\to\pi/2} \frac{\sin t - \sin(\pi/2)}{t-\pi/2}
    \end{displaymath}
    which is an alternate form for the derivative of $f(t)=\sin t$ at
    $a=\pi/2$.
    
    Alternatively, you can convert the limit so it is a limit as
    $h\to 0$.  Let $h=t-\pi/2$, in which case $t=h + \pi/2$.  We have
    \begin{align*}
      \lim_{t\to\pi/2} \frac{\sin t - 1}{t-\pi/2}
      &= \lim_{h\to 0} \frac{\sin(h+\pi/2)-\sin(\pi/2)}{h}
    \end{align*}
    so we have $f(t)=\sin t$ and $a=\pi/2$.
  \end{enumerate}
\item %9
  In business applications, the derivative is usually interpreted
  as the ``marginal''.
  \begin{enumerate}
  \item The marginal cost is the cost of making one more widget after
    you have made $x$ widgets.  It can be written as
    \begin{equation*}
      f(x+1) - f(x) = \frac{f(x+1)-f(x)}{1} = \frac{f(x+h)-f(x)}{h}
    \end{equation*}
    where $h=1$.  If you are making large numbers of widgets, $1$ is
    considered close to $0$, so we have the approximation
    \begin{equation*}
      f'(x) = \lim_{h\to 0} \frac{f(x+h)-f(x)}{h} \approx
      \frac{f(x+1)-f(x)}{1}
    \end{equation*}
    so the derivative is approximately equal to the marginal.  The
    units are dollars per widget.
  \item $f'(100)=12$ means the cost of making one more widget, after
    you have already made 100 widgets, is 12 dollars.  (Usually the
    first few widgets are very expensive because they carry the fixed
    costs like renting factory space, etc.  After you get rolling, the
    cost of one more widget just includes the materials and labour,
    not the fixed costs.)
  \item For small values of $x$, the marginal cost will decrease as
    you make more widgets, because more of the fixed costs will be
    absorbed into the previously made widgets.  For large values of
    $x$ we may see an increase in the marginal cost because extra
    manufacturing capacity will need to be added beyond a certain
    level, and materials costs will increase because of the increasing
    demand caused by your manufacturing.
  \end{enumerate}
\item %10
  This question is hard.  When $x\ne 0$,
  \begin{align*}
    f(0+h) &= (0+h)^2 \cos \frac{1}{0+h}
    \\
    f(0) &= 0
  \end{align*}
  where we have used the first part of the definition of $f$ for
  values $x=0+h$ away from $0$, and the second part of the definition
  of $f$ for the value $x=0$.
  \begin{align*}
    \\
    f(0+h) - f(0) &= h^2 \cos \frac{1}{h}
    \\
    \frac{f(0+h)-f(0)}{h} &= h \cos \frac{1}{h}
    \\
    f'(0) &= \lim_{h\to 0} \frac{f(0+h)-f(0)}{h}
            = \lim_{h\to 0} h \cos \frac{1}{h}
  \end{align*}
  We have to be careful evaluating this limit.  We can't use the
  product rule for limits because
  \begin{equation*}
    \lim_{h\to 0} \cos \frac{1}{h}
  \end{equation*}
  does not exist.  Instead we have to use the squeeze theorem.  Note
  that $\cos$ is bounded between $-1$ and $1$:
  \begin{equation*}
    -1 \le \cos \frac{1}{h} \le 1
  \end{equation*}
  for any $h\ne 0$.  Assuming $h>0$, multiply by $h$ to obtain
  \begin{equation*}
    -h \le h \cos \frac{1}{h} \le h
  \end{equation*}
  Both $-h\to 0$ and $h\to 0$, squeezing the value in the middle, so
  we can conclude that the one sided limit
  \begin{equation*}
    \lim_{h\to 0^+} h \cos \frac{1}{h} = 0
  \end{equation*}
  You should make a similar (but slightly different) argument to show
  that $\lim_{h\to 0^-} h\cos (1/h) = 0$ also.  Since the one-sided
  limits exist and are equal, we conclude that
  \begin{equation*}
    f'(0) = \lim_{h\to 0} h \cos \frac{1}{h} = 0
  \end{equation*}
\end{enumerate}
\end{document}



%%%%%%%%%%%%%%%%%%%%%%%%%%%%%%%%%%%%%%%%%%%%%%%%%%%%%%%%%%%%%%%%%%%%%%
%%% MATH110-PS021-Solutions.tex ends here
