\documentclass{article}
\usepackage{fullpage}
\usepackage{mathptmx}
\usepackage{graphicx}
\usepackage{amsmath}
\usepackage[aux]{rerunfilecheck}

\newcommand{\ds}{\displaystyle}

\input{../common.tex}

\title{MATH 110 Midterm Test 2 Solutions}
\author{\commonAuthor}
\date{\commonDateMTTwo}

\begin{document}
\maketitle

\section{A Version}

\begin{enumerate}
\item
  \begin{enumerate}
  \item We can write $y=(\tan(3x))^2$, so $y$ is the composition of three
    functions.  We have 
    \begin{align*}
      \frac{dy}{dx} = 2(\tan(3x))^1 \cdot \frac{d}{dx} \tan(3x)
      = 2\tan(3x) \sec^2(3x) \frac{d}{dx} 3x
      = 2\tan(3x) \cdot \sec^2(3x) \cdot 3
    \end{align*}
  \item We can write $g(t)=(t^2+1)^{1/3}$ so we have by the chain rule
    \begin{align*}
      g'(t) = \frac{1}{3} (t^2+1)^{-2/3} \cdot \frac{d}{dt} (t^2+1)
      = \frac{1}{3} (t^2+1)^{-2/3} \cdot 2t
      = \frac{2}{3} t(t^2+1)^{-2/3}
    \end{align*}
    Differentiating again, by the product rule and the chain rule,
    \begin{align*}
      g''(t) = \frac{2}{3} (t^2+1)^{-2/3} 
      + \frac{2}{3} t \frac{d}{dt} (t^2+1)^{-2/3}
      = \frac{2}{3} (t^2+1)^{-2/3} 
      + \frac{2}{3} t \cdot -\frac{2}{3}(t^2+1)^{-5/3} \cdot 2t
    \end{align*}
  \end{enumerate}
\item By the quotient rule we have
  \begin{align*}
    \frac{dy}{ds} = \frac{(1+2s)-s(2)}{(1+2s)^2}
    = \frac{1}{(1+2s)^2}
  \end{align*}
  so
  \begin{align*}
    dy = \frac{1}{(1+2s)^2} \; ds
  \end{align*}
\item Multiplying and dividing by the conjugate radical we have
  \begin{align*}
    \lim_{x\to\infty} \left(\sqrt{4x^2+2x}-2x\right)
    = \lim_{x\to\infty} \left(\sqrt{4x^2+2x}-2x\right)
    \cdot \frac{\sqrt{4x^2+2x}+2x}{\sqrt{4x^2+2x}+2x}
    = \lim_{x\to\infty} \frac{2x}{\sqrt{4x^2+2x}+2x}
  \end{align*}
  Dividing through by the highest power of $x$ in the denominator, namely
  $x$ (because $x^2$ appears under the square root sign),
  \begin{align*}
    \lim_{x\to\infty} \frac{2x}{\sqrt{4x^2+2x}+2x}
    = \lim_{x\to\infty} \frac{2}{\sqrt{4x^2/x^2 + 2x/x^2} + 2}
    = \lim_{x\to\infty} \frac{2}{\sqrt{4+2/x}+2}
    = \frac{2}{\sqrt{4+0}+2}
    = \frac{1}{2}
  \end{align*}
\item 
  \begin{enumerate}
  \item Call the short side $x$ and the height $h$; then the long side is
    $2x$.  See Figure~\ref{fig:boxa}.
    \begin{figure}[htbp]
      \begin{center}
      $\begin{array}{c@{\hspace{1in}}c}
      \includegraphics[width=2in]{boxa.eps}
      &
      \includegraphics[width=2in]{unboxa.eps}
      \\
      \mbox{(a) oblique projection}
      &
      \mbox{(b) unfolded}
      \end{array}$
      \end{center}
      \caption{Two views of the box}
      \label{fig:boxa}
    \end{figure}
  \item The amount of material on the base is $x\times 2x=2x^2$, the
    amount of material on the short sides is $xh+xh=2xh$, and the amount
    of material on the long sides is $2xh+2xh=4xh$, so the objective
    function to be minimized is $S=2x^2+6xh$.  The constraint is that
    the volume must be 10 units, so $10=x\cdot 2x\cdot h$ or $10=2x^2h$.
  \item We use the constraint to eliminate one of the variables.  The
    easiest way is to write $h=5/x^2$, so
    $S(x) = 2x^2 + 30/x$
    is to be minimized.  Its first derivative is $S'(x)=4x-30/x^2$ so a
    local minimum will occur when $S'(x)$ is undefined (nowhere) or 
    when $S'(x)=0$ which is equivalent to $x^3=7.5$ or $x=\sqrt[3]{7.5}$.

    To apply the first derivative test note $S'(x)=(4x^3-30)/x^2$ is
    negative when $4x^3-30<0$, i.e., when $x<\sqrt[3]{7.5}$, and is
    positive when $4x^3-30>0$, i.e., when $x>\sqrt[3]{7.5}$.  Therefore
    $S(x)$ decreases from $0$ to $\sqrt[3]{7.5}$ then increases thereafter,
    guaranteeing that $S(x)$ has a global minimum at $x=\sqrt[3]{7.5}$.
  \item The dimensions of the box which minimize the amount of material
    used are $\sqrt[3]{7.5}$ for the short side, $2\sqrt[3]{7.5}$ for the
    long side, and $5/(\sqrt[3]{7.5})^2$ for the height.
  \end{enumerate}
\item Call the point at which the cars start the origin.  
  The distance between the cars always satisfies $z^2=x^2+y^2$, so the
  rates of change are related by $zz'=xx'+yy'$.
  Two hours later,
  we have the car moving south at position $y=-120$ and the car moving west
  at position $x=-50$.  The distance between the cars is $z=\sqrt{(-50)^2
  +(-120)^2}= 130$ and the known velocities are $y'=-60$ and $x'=-25$.
  Filling in all that information we have
  \begin{align*}
    z' = \frac{xx'+yy'}{z}
    = \frac{-50\cdot -25 + -120\cdot -60}{130} = 65
  \end{align*}
  Two hours later, the distance between the cars is increasing at a rate
  of $65$ mi/h.
\item Note that $f'(x)$ is negative when $x<1$ and positive when $1<x$,
  so $f(x)$ is decreasing when $x<1$ and increasing when $1<x$.  Similarly,
  $f''(x)$ is negative when $x<0$, positive when $0<x<2$, and negative
  when $2<x$, so $f(x)$ is concave down when $x<0$, concave up when
  $0<x<2$, and concave down when $2<x$.
  \begin{enumerate}
  \item $f$ is increasing and concave up on the overlap of the intervals
    on which it is increasing ($1<x$) and concave up ($0<x<2$), i.e.,
    $f$ is increasing and concave up on $1<x<2$.
  \item $f$ is increasing and concave down on $2<x$.
  \item $f$ is decreasing and concave up when $0<x<1$.
  \item $f$ is decreasing and concave down when $x<0$.
  \item We have $\ds \lim_{x\to\pm\infty} f(x) = 
    \lim_{x\to\pm\infty} \frac{2-4/x+1/x^2}{1-2/x+4/x^2} = 2$, so the
    horizontal asymptote is $y=2$.
  \end{enumerate}
  See Figure~\ref{fig:fa}.  Although the graph isn't required to answer
  the question, graphing the function makes it easier to understand and
  visualize the situation.
  \begin{figure}[htbp]
    \begin{center}
      \includegraphics[width=6in]{fa.eps}
    \end{center}
    \caption{Graph of $f(x)=(2x^2-4x+1)/(x^2-2x+4)$}
    \label{fig:fa}
  \end{figure}
\item \textbf{Solution 1:} Multiplying and dividing by the ``conjugate''
  $\cos\theta + 1$ and using $\tan\theta = \sin\theta/\cos\theta$,
  \begin{align*}
    \lim_{\theta\to 0} \frac{\cos\theta-1}{\tan\theta}
    = \lim_{\theta\to 0} 
    \frac{(\cos\theta-1)(\cos\theta+1)\cos\theta}{\sin\theta(\cos\theta+1)}
    = \lim_{\theta\to 0} 
    \frac{(\cos^2\theta-1)\cos\theta}{\sin\theta(\cos\theta+1)}
  \end{align*}
  Using the Pythagorean identity $\sin^2\theta + \cos^2\theta=1$,
  \begin{align*}
    \lim_{\theta\to 0} 
    \frac{(\cos^2\theta-1)\cos\theta}{\sin\theta(\cos\theta+1)}
    = \lim_{\theta\to 0} 
    \frac{-\sin^2\theta\cos\theta}{\sin\theta(\cos\theta+1)}
    = \lim_{\theta\to 0}
    \frac{-\sin\theta\cos\theta}{\cos\theta+1}
    = \frac{-0\cdot 1}{1+1} = 0
  \end{align*}

  \textbf{Solution 2:} Using the identity $\tan\theta = \sin\theta/\cos\theta$
  and multiplying and dividing by $\theta$ gives
  \begin{align*}
    \lim_{\theta\to 0} \frac{\cos\theta-1}{\tan\theta}
    = \lim_{\theta\to 0} \frac{\cos\theta-1}{\theta}
    \cdot \frac{\theta}{\sin\theta} \cdot \cos\theta
    = \lim_{\theta\to 0} \frac{\cos\theta-1}{\theta}
    \cdot \lim_{\theta\to 0}\frac{\theta}{\sin\theta} \cdot 
    \lim_{\theta\to 0} \cos\theta
    = 0 \cdot 1 \cdot 1 = 0
  \end{align*}
  by the basic trig limits.
\item We have to show that the function $\ds f(x)=2\sqrt{x}-3+1/x$ satisfies
  $f(x)>0$ for all $x>1$.  Note
  $f'(x)=x^{-1/2} - 1/x^2 = (x^{3/2}-1)/x^2 >0$ for $x>1$ so $f(x)$ is 
  increasing for $x>1$, which means $f(x)>f(1)=0$ for $x>1$, as required.
\end{enumerate}


\section{B Version}

\begin{enumerate}
\item
  \begin{enumerate}
  \item We can write $y=(\sec(2x))^3$, so $y$ is the composition of three
    functions.  We have 
    \begin{align*}
      \frac{dy}{dx} = 3(\sec(2x))^2 \cdot \frac{d}{dx} \sec(2x)
      = 3\sec^2(2x) \sec(2x)\tan(2x) \frac{d}{dx} 2x
      = 3\sec^2(2x) \cdot \sec(2x)\tan(2x) \cdot 2
    \end{align*}
  \item We can write $g(t)=(t^3+1)^{1/2}$ so we have by the chain rule
    \begin{align*}
      g'(t) = \frac{1}{2} (t^3+1)^{-1/2} \cdot \frac{d}{dt} (t^3+1)
      = \frac{1}{2} (t^3+1)^{-1/2} \cdot 3t^2
      = \frac{3}{2} t^2(t^3+1)^{-1/2}
    \end{align*}
    Differentiating again, by the product rule and the chain rule,
    \begin{align*}
      g''(t) = \frac{3}{2} 2t (t^3+1)^{-1/2} 
      + \frac{3}{2} t^2 \frac{d}{dt} (t^3+1)^{-1/2}
      = 3t (t^3+1)^{-1/2} 
      + \frac{3}{2} t^2 \cdot -\frac{1}{2} (t^3+1)^{-3/2} \cdot 3t^2
    \end{align*}
  \end{enumerate}
\item By the quotient rule we have
  \begin{align*}
    \frac{dy}{du} = \frac{(u-1)-(u+1)}{(u-1)^2}
    = \frac{-2}{(u-1)^2}
  \end{align*}
  so
  \begin{align*}
    dy = -\frac{2}{(u-1)^2} \; du
  \end{align*}
\item Multiplying and dividing by the conjugate radical we have
  \begin{align*}
    \lim_{x\to\infty} \left(\sqrt{9x^2+x}-3x\right)
    = \lim_{x\to\infty} \left(\sqrt{9x^2+x}-3x\right)
    \cdot \frac{\sqrt{9x^2+x}+3x}{\sqrt{9x^2+x}+3x}
    = \lim_{x\to\infty} \frac{x}{\sqrt{9x^2+x}+3x}
  \end{align*}
  Dividing through by the highest power of $x$ in the denominator, namely
  $x$ (because $x^2$ appears under the square root sign),
  \begin{align*}
    \lim_{x\to\infty} \frac{x}{\sqrt{9x^2+x}+3x}
    = \lim_{x\to\infty} \frac{1}{\sqrt{9x^2/x^2 + x/x^2} + 3x/x}
    = \lim_{x\to\infty} \frac{1}{\sqrt{9+1/x}+3}
    = \frac{1}{\sqrt{9+0}+3}
    = \frac{1}{6}
  \end{align*}
\item 
  \begin{enumerate}
  \item Call the short side $x$ and the height $h$; then the long side is
    $3x$.  See Figure~\ref{fig:boxb}.
    \begin{figure}[htbp]
      \begin{center}
      $\begin{array}{c@{\hspace{1in}}c}
      \includegraphics[width=2in]{boxb.eps}
      &
      \includegraphics[width=2in]{unboxb.eps}
      \\
      \mbox{(a) oblique projection}
      &
      \mbox{(b) unfolded}
      \end{array}$
      \end{center}
      \caption{Two views of the box}
      \label{fig:boxb}
    \end{figure}
  \item The amount of material on the base is $x\times 3x=3x^2$, the
    amount of material on the short sides is $xh+xh=2xh$, and the amount
    of material on the long sides is $3xh+3xh=6xh$, so the objective
    function to be minimized is $S=3x^2+8xh$.  The constraint is that
    the volume must be 10 units, so $10=x\cdot 3x\cdot h$ or $10=3x^2h$.
  \item We use the constraint to eliminate one of the variables.  The
    easiest way is to write $h=10/(3x^2)$, so
    $S(x) = 3x^2 + 80/(3x)$
    is to be minimized.  Its first derivative is $S'(x)=6x-80/(3x^2)$ so a
    local minimum will occur when $S'(x)$ is undefined (nowhere) or 
    when $S'(x)=0$ which is equivalent to $x^3=40/9$ or $x=\sqrt[3]{40/9}$.

    To apply the first derivative test note $S'(x)=(18x^3-80)/x^2$ is
    negative when $18x^3-80<0$, i.e., when $x<\sqrt[3]{40/9}$, and is
    positive when $18x^3-80>0$, i.e., when $x>\sqrt[3]{40/9}$.  Therefore
    $S(x)$ decreases from $0$ to $\sqrt[3]{40/9}$ then increases thereafter,
    guaranteeing that $S(x)$ has a global minimum at $x=\sqrt[3]{40/9}$.
  \item The dimensions of the box which minimize the amount of material
    used are $\sqrt[3]{40/9}$ for the short side, $2\sqrt[3]{40/9}$ for the
    long side, and $10/(3(\sqrt[3]{40/9})^2)$ for the height.
  \end{enumerate}
\item Call the point at which the cars start the origin.  
  The distance between the cars always satisfies $z^2=x^2+y^2$, so the
  rates of change are related by $zz'=xx'+yy'$.
  Two hours later,
  we have the car moving north at position $y=120$ and the car moving east
  at position $x=160$.  The distance between the cars is $z=\sqrt{(160)^2
  +(120)^2}= 200$ and the known velocities are $y'=60$ and $x'=80$.
  Filling in all that information, we have
  \begin{align*}
    z' = \frac{xx'+yy'}{z}
    = \frac{160\cdot 80 + 120\cdot 60}{200} = 100
  \end{align*}
  Two hours later, the distance between the cars is increasing at a rate
  of $100$ mi/h.
\item Note that $f'(x)$ is negative when $x<0$ and positive when $0<x$,
  so $f(x)$ is decreasing when $x<0$ and increasing when $0<x$.  Similarly,
  $f''(x)$ is negative when $x<-1$, positive when $-1<x<1$, and negative
  when $1<x$, so $f(x)$ is concave down when $x<-1$, concave up when
  $-1<x<1$, and concave down when $1<x$.
  \begin{enumerate}
  \item $f$ is increasing and concave up on the overlap of the intervals
    on which it is increasing ($0<x$) and concave up ($-1<x<1$), i.e.,
    $f$ is increasing and concave up on $0<x<1$.
  \item $f$ is increasing and concave down on $1<x$.
  \item $f$ is decreasing and concave up when $-1<x<0$.
  \item $f$ is decreasing and concave down when $x<-1$.
  \item We have $\ds \lim_{x\to\pm\infty} f(x) = 
    \lim_{x\to\pm\infty} \frac{1+1/x^2}{1+3/x^2} = 1$, so the
    horizontal asymptote is $y=1$.
  \end{enumerate}
  See Figure~\ref{fig:fb}.  Although the graph isn't required to answer
  the question, graphing the function makes it easier to understand and
  visualize the situation.
  \begin{figure}[htbp]
    \begin{center}
      \includegraphics[width=6in]{fb.eps}
    \end{center}
    \caption{Graph of $f(x)=(x^2+1)/(x^2+3)$}
    \label{fig:fb}
  \end{figure}
\item \textbf{Solution 1:} Multiplying and dividing by the ``conjugate''
  $\cos\theta + 1$ and using $\tan\theta = \sin\theta/\cos\theta$,
  \begin{align*}
    \lim_{\theta\to 0} \frac{\cos\theta-1}{\tan\theta}
    = \lim_{\theta\to 0} 
    \frac{(\cos\theta-1)(\cos\theta+1)\cos\theta}{\sin\theta(\cos\theta+1)}
    = \lim_{\theta\to 0} 
    \frac{(\cos^2\theta-1)\cos\theta}{\sin\theta(\cos\theta+1)}
  \end{align*}
  Using the Pythagorean identity $\sin^2\theta + \cos^2\theta=1$,
  \begin{align*}
    \lim_{\theta\to 0} 
    \frac{(\cos^2\theta-1)\cos\theta}{\sin\theta(\cos\theta+1)}
    = \lim_{\theta\to 0} 
    \frac{-\sin^2\theta\cos\theta}{\sin\theta(\cos\theta+1)}
    = \lim_{\theta\to 0}
    \frac{-\sin\theta\cos\theta}{\cos\theta+1}
    = \frac{-0\cdot 1}{1+1} = 0
  \end{align*}

  \textbf{Solution 2:} Using the identity $\tan\theta = \sin\theta/\cos\theta$
  and multiplying and dividing by $\theta$ gives
  \begin{align*}
    \lim_{\theta\to 0} \frac{\cos\theta-1}{\tan\theta}
    = \lim_{\theta\to 0} \frac{\cos\theta-1}{\theta}
    \cdot \frac{\theta}{\sin\theta} \cdot \cos\theta
    = \lim_{\theta\to 0} \frac{\cos\theta-1}{\theta}
    \cdot \lim_{\theta\to 0}\frac{\theta}{\sin\theta} \cdot 
    \lim_{\theta\to 0} \cos\theta
    = 0 \cdot 1 \cdot 1 = 0
  \end{align*}
  by the basic trig limits.
\item We have to show that the function $\ds f(x)=2\sqrt{x}-3+1/x$ satisfies
  $f(x)>0$ for all $x>1$.  Note
  $f'(x)=x^{-1/2} - 1/x^2 = (x^{3/2}-1)/x^2 >0$ for $x>1$ so $f(x)$ is 
  increasing for $x>1$, which means $f(x)>f(1)=0$ for $x>1$, as required.
\end{enumerate}


\section{C Version}

\begin{enumerate}
\item
  \begin{enumerate}
  \item We can write $y=(\sec(3x))^2$, so $y$ is the composition of three
    functions.  We have 
    \begin{align*}
      \frac{dy}{dx} = 2(\sec(3x))^1 \cdot \frac{d}{dx} \sec(3x)
      = 2\sec(3x) \sec(3x)\tan(3x) \frac{d}{dx} 3x
      = 2\sec(3x) \cdot \sec(3x)\tan(3x) \cdot 3
    \end{align*}
  \item We can write $g(t)=(t^2+1)^{1/2}$ so we have by the chain rule
    \begin{align*}
      g'(t) = \frac{1}{2} (t^2+1)^{-1/2} \cdot \frac{d}{dt} (t^2+1)
      = \frac{1}{2} (t^2+1)^{-1/2} \cdot 2t
      = t(t^2+1)^{-1/2}
    \end{align*}
    Differentiating again, by the product rule and the chain rule,
    \begin{align*}
      g''(t) = (t^2+1)^{-1/2} 
      + t \frac{d}{dt} (t^2+1)^{-1/2}
      = (t^2+1)^{-1/2} 
      + t \cdot -\frac{1}{2}(t^2+1)^{-3/2} \cdot 2t
    \end{align*}
  \end{enumerate}
\item By the quotient rule we have
  \begin{align*}
    \frac{dy}{dx} = \frac{(x+1)-(x-1)}{(x+1)^2}
    = \frac{2}{(x+1)^2}
  \end{align*}
  so
  \begin{align*}
    dy = \frac{2}{(x+1)^2} \; dx
  \end{align*}
\item Multiplying and dividing by the conjugate radical we have
  \begin{align*}
    \lim_{x\to\infty} \left(\sqrt{25x^2+3x}-5x\right)
    = \lim_{x\to\infty} \left(\sqrt{25x^2+3x}-5x\right)
    \cdot \frac{\sqrt{25x^2+3x}+5x}{\sqrt{25x^2+3x}+5x}
    = \lim_{x\to\infty} \frac{3x}{\sqrt{25x^2+3x}+5x}
  \end{align*}
  Dividing through by the highest power of $x$ in the denominator, namely
  $x$ (because $x^2$ appears under the square root sign),
  \begin{align*}
    \lim_{x\to\infty} \frac{3x}{\sqrt{25x^2+3x}+5x}
    = \lim_{x\to\infty} \frac{3}{\sqrt{25x^2/x^2 + 3x/x^2} + 5}
    = \lim_{x\to\infty} \frac{3}{\sqrt{25+3/x}+5}
    = \frac{3}{\sqrt{25+0}+5}
    = \frac{3}{10}
  \end{align*}
\item 
  \begin{enumerate}
  \item Call the short side $x$ and the height $h$; then the long side is
    $4x$.  See Figure~\ref{fig:boxc}.
    \begin{figure}[htbp]
      \begin{center}
      $\begin{array}{c@{\hspace{1in}}c}
      \includegraphics[width=2in]{boxc.eps}
      &
      \includegraphics[width=2in]{unboxc.eps}
      \\
      \mbox{(a) oblique projection}
      &
      \mbox{(b) unfolded}
      \end{array}$
      \end{center}
      \caption{Two views of the box}
      \label{fig:boxc}
    \end{figure}
  \item The amount of material on the base is $x\times 4x=4x^2$, the
    amount of material on the short sides is $xh+xh=2xh$, and the amount
    of material on the long sides is $4xh+4xh=8xh$, so the objective
    function to be minimized is $S=4x^2+10xh$.  The constraint is that
    the volume must be 10 units, so $10=x\cdot 4x\cdot h$ or $10=4x^2h$.
  \item We use the constraint to eliminate one of the variables.  The
    easiest way is to write $h=5/(2x^2)$, so
    $S(x) = 4x^2 + 25/x$
    is to be minimized.  Its first derivative is $S'(x)=8x-25/x^2$ so a
    local minimum will occur when $S'(x)$ is undefined (nowhere) or 
    when $S'(x)=0$ which is equivalent to $x^3=25/8$ or $x=\sqrt[3]{25/8}$.

    To apply the first derivative test note $S'(x)=(8x^3-25)/x^2$ is
    negative when $8x^3-25<0$, i.e., when $x<\sqrt[3]{25/8}$, and is
    positive when $8x^3-25>0$, i.e., when $x>\sqrt[3]{25/8}$.  Therefore
    $S(x)$ decreases from $0$ to $\sqrt[3]{25/8}$ then increases thereafter,
    guaranteeing that $S(x)$ has a global minimum at $x=\sqrt[3]{25/8}$.
  \item The dimensions of the box which minimize the amount of material
    used are $\sqrt[3]{25/8}$ for the short side, $4\sqrt[3]{25/8}$ for the
    long side, and $5/(2(\sqrt[3]{25/8})^2)$ for the height.
  \end{enumerate}
\item Call the point at which the cars start the origin.  
  The distance between the cars always satisfies $z^2=x^2+y^2$, so the
  rates of change are related by $zz'=xx'+yy'$.
  Two hours later,
  we have the car moving north at position $y=200$ and the car moving west
  at position $x=-150$.  The distance between the cars is $z=\sqrt{(-150)^2
  +(200)^2}= 250$ and the known velocities are $y'=100$ and $x'=-75$.
  Filling in all that information we have
  \begin{align*}
    z' = \frac{xx'+yy'}{z}
    = \frac{-150\cdot -75 + 200\cdot 100}{250} = 125
  \end{align*}
  Two hours later, the distance between the cars is increasing at a rate
  of $125$ km/h.
\item Note that $f'(x)$ is negative when $x<-1$ and positive when $-1<x$,
  so $f(x)$ is decreasing when $x<-1$ and increasing when $-1<x$.  Similarly,
  $f''(x)$ is negative when $x<-2$, positive when $-2<x<0$, and negative
  when $0<x$, so $f(x)$ is concave down when $x<-2$, concave up when
  $-20<x<0$, and concave down when $0<x$.
  \begin{enumerate}
  \item $f$ is increasing and concave up on the overlap of the intervals
    on which it is increasing ($-1<x$) and concave up ($-2<x<0$), i.e.,
    $f$ is increasing and concave up on $-1<x<0$.
  \item $f$ is increasing and concave down on $0<x$.
  \item $f$ is decreasing and concave up when $-2<x<-1$.
  \item $f$ is decreasing and concave down when $x<-2$.
  \item We have $\ds \lim_{x\to\pm\infty} f(x) = 
    \lim_{x\to\pm\infty} \frac{1-2/x}{1+2/x+4/x^2} = 1$, so the
    horizontal asymptote is $y=1$.
  \end{enumerate}
  See Figure~\ref{fig:fc}.  Although the graph isn't required to answer
  the question, graphing the function makes it easier to understand and
  visualize the situation.
  \begin{figure}[htbp]
    \begin{center}
      \includegraphics[width=6in]{fc.eps}
    \end{center}
    \caption{Graph of $f(x)=(x^2+2x)/(x^2+2x+4)$}
    \label{fig:fc}
  \end{figure}
\item \textbf{Solution 1:} Multiplying and dividing by the ``conjugate''
  $\cos\theta + 1$ and using $\tan\theta = \sin\theta/\cos\theta$,
  \begin{align*}
    \lim_{\theta\to 0} \frac{\cos\theta-1}{\tan\theta}
    = \lim_{\theta\to 0} 
    \frac{(\cos\theta-1)(\cos\theta+1)\cos\theta}{\sin\theta(\cos\theta+1)}
    = \lim_{\theta\to 0} 
    \frac{(\cos^2\theta-1)\cos\theta}{\sin\theta(\cos\theta+1)}
  \end{align*}
  Using the Pythagorean identity $\sin^2\theta + \cos^2\theta=1$,
  \begin{align*}
    \lim_{\theta\to 0} 
    \frac{(\cos^2\theta-1)\cos\theta}{\sin\theta(\cos\theta+1)}
    = \lim_{\theta\to 0} 
    \frac{-\sin^2\theta\cos\theta}{\sin\theta(\cos\theta+1)}
    = \lim_{\theta\to 0}
    \frac{-\sin\theta\cos\theta}{\cos\theta+1}
    = \frac{-0\cdot 1}{1+1} = 0
  \end{align*}

  \textbf{Solution 2:} Using the identity $\tan\theta = \sin\theta/\cos\theta$
  and multiplying and dividing by $\theta$ gives
  \begin{align*}
    \lim_{\theta\to 0} \frac{\cos\theta-1}{\tan\theta}
    = \lim_{\theta\to 0} \frac{\cos\theta-1}{\theta}
    \cdot \frac{\theta}{\sin\theta} \cdot \cos\theta
    = \lim_{\theta\to 0} \frac{\cos\theta-1}{\theta}
    \cdot \lim_{\theta\to 0}\frac{\theta}{\sin\theta} \cdot 
    \lim_{\theta\to 0} \cos\theta
    = 0 \cdot 1 \cdot 1 = 0
  \end{align*}
  by the basic trig limits.
\item We have to show that the function $\ds f(x)=2\sqrt{x}-3+1/x$ satisfies
  $f(x)>0$ for all $x>1$.  Note
  $f'(x)=x^{-1/2} - 1/x^2 = (x^{3/2}-1)/x^2 >0$ for $x>1$ so $f(x)$ is 
  increasing for $x>1$, which means $f(x)>f(1)=0$ for $x>1$, as required.
\end{enumerate}

\end{document}

