\documentclass[12pt]{article}
\usepackage{mathptmx}
\usepackage{fullpage}
\usepackage{multicol}
\usepackage{amsmath,amssymb}
\usepackage[aux]{rerunfilecheck}

\newcommand{\ds}{\displaystyle}

\reversemarginpar

\title{MATH110--S01--S02 200930 Quiz 3 Solutions}
\author{Edward Doolittle}

\begin{document}
\maketitle

\begin{enumerate}
\item To find the equation of the tangent line in point-slope form we need
  to find a point $(x_0,y_0)$ through which the tangent line passes and
  we need to find
  the slope of the tangent line.  The point is given: $(4,10)$ (though it's
  a good idea to check that that point really is on the curve).  So we now need
  to find the slope of the tangent line.  The slope of the tangent line
  is the derivative $y'$ evaluated at $x=4$.  By the product rule we have
  \begin{equation*}
    y' = \frac{d}{dx} \left(x^{1/2} (x+1)\right)
    = \left(\frac{d}{dx} x^{1/2} \right) (x+1) 
    + x^{1/2} \left(\frac{d}{dx} (x+1) \right)
    = \frac{1}{2} x^{-1/2} (x+1) + x^{1/2} \cdot 1
  \end{equation*}
  so
  \begin{equation*}
    m = y'(4) = \frac{1}{2} 4^{-1/2} (4+1) + 4^{1/2} \cdot 1
    = \frac{1}{2} \frac{1}{\sqrt{4}} (5) + \sqrt{4}
    = \frac{5}{4} + 2 = \frac{13}{4} 
  \end{equation*}
  Assembling all the information, the equation of the tangent line is
  \begin{equation*}
    y-10 = \frac{13}{4}(x-4)
  \end{equation*}
\item The first derivative of $f$ is
  \begin{equation*}
    f'(x) = \frac{\left(\frac{d}{dx} 1\right)(2-x) 
    - 1 \frac{d}{dx} (2-x)}{(2-x)^2}
    = \frac{1}{(2-x)^2}
  \end{equation*}
  so the second derivative of $f$ is
  \begin{align*}
    f''(x) 
    &= \frac{d}{dx} \frac{1}{(2-x)^2}
    = \frac{\left(\frac{d}{dx} 1\right)(2-x)^2 - 1\frac{d}{dx} (2-x)^2}{(2-x)^4}
    \\
    &= \frac{-2(2-x)\frac{d}{dx}(2-x)}{(2-x)^4}
    = \frac{2(2-x)}{(2-x)^4}
    = \frac{2}{(2-x)^3}
  \end{align*}
\end{enumerate}

\end{document}


