\documentclass[12pt]{article}
\usepackage{mathptmx}
\usepackage{fullpage}
\usepackage{multicol}
\usepackage{amsmath,amssymb}
\usepackage[aux]{rerunfilecheck}

\newcommand{\ds}{\displaystyle}

\reversemarginpar

\title{MATH 110-004 200730 Quiz 3 Solutions}
\author{Edward Doolittle}

\begin{document}
\maketitle

\begin{enumerate}
\item By the product rule and the chain rule,
  \begin{align*}
    f'(a) = 2a \cos \frac{1}{a} 
      + a^2 \cdot -\sin \frac{1}{a} \frac{d}{da} a^{-1}
      = 2a \cos \frac{1}{a} - a^2 \sin \frac{1}{a} \cdot -a^{-2}
      = 2a \cos \frac{1}{a} + \sin \frac{1}{a}
  \end{align*}
  The answer applies for all values of $a$ in the domain of $f$ where it
  makes sense, i.e., for all $a\ne 0$.
\item The tangent is horizontal where $y'=0$, so we calculate the
  derivative and set it equal to $0$:
  \begin{align*}
    y' = \frac{(2+\cos x)\cos x - \sin x \cdot -\sin x}{(2+\cos x)^2}
    = \frac{2\cos x + \cos^2 x + \sin^2 x}{(2+\cos x)^2}
    = \frac{2\cos x + 1}{(2+\cos x)^2}
  \end{align*}
  where the Pythagorean identity $\cos^2 x + \sin^2 x = 1$ was used to
  simplify the result.  Then $y'=0$ implies
  \begin{align*}
    \frac{2\cos x + 1}{(2+\cos x)^2} = 0
    \implies 2\cos x + 1 = 0
    \implies x = \pm \frac{2\pi}{3} + 2k\pi, k=0, \pm 1, \pm 2, \ldots
  \end{align*}
\end{enumerate}

\end{document}


