\documentclass{article}
% \usepackage{fullpage}
\usepackage{amsmath}
\usepackage[margin=0.5in]{geometry}
% \usepackage{mathptmx}
% \usepackage{txfonts}
\usepackage{multicol}
\usepackage{pgfplots}
\pgfplotsset{compat=1.17}
\usepgfplotslibrary{fillbetween}
\usepackage[aux]{rerunfilecheck}
\usepackage{tikz}
\usetikzlibrary{calc}

\newcommand{\ds}{\displaystyle}

\input{../common.tex}

\title{\commonPSTitleZeroFourTwo\ Solutions}
\author{\commonAuthor}
\date{\commonDateZeroFourTwo}

\begin{document}
\maketitle
\thispagestyle{empty}

\noindent
\begin{enumerate}
\item % (Based on 4.2.22--24)
  \begin{enumerate}
  \item Note that $a=1$, $b=4$, and
    $f(x)=x^2+2x-5$.  First, we calculate $\Delta x$:
    \begin{equation*}
      \Delta x = \frac{b-a}{n} = \frac{4-1}{n} = \frac{3}{n}
    \end{equation*}
    Now we find $x_i$, the boundaries of the sub-intervals:
    \begin{equation*}
      x_i = a + i \Delta x = 1 + i \frac{3}{n} = 1 + \frac{3i}{n}
    \end{equation*}
    Now we are ready to write the definite integral as a limit of
    Riemann sums:
    \begin{align*}
      \int_1^4 (x^2+2x-5) \; dx
      &= \lim_{n\to\infty} \sum_{i=1}^n (x_i^2+2x_i-5)\; \Delta x \\
      &= \lim_{n\to\infty} \sum_{i=1}^n \left( \left(1+\frac{3i}{n}\right)^2 +
        2\left(1+\frac{3i}{n}\right) - 5 \right) \; \frac{3}{n} \\
      &= \lim_{n\to\infty} \frac{3}{n} \sum_{i=1}^n \left( 1 + \frac{6i}{n} +
        \frac{9i^2}{n^2} + 2 + \frac{6i}{n} - 5 \right) 
      \\
      &= \lim_{n\to\infty} \frac{3}{n} \sum_{i=1}^n \left( -2 + \frac{12}{n} i +
        \frac{9}{n^2} i^2\right)
      \\
      &= \lim_{n\to\infty} \frac{3}{n} \left(\sum_{i=1}^n -2
        + \sum_{i=1}^n \frac{12}{n} i + \sum_{i=1}^n \frac{9}{n^2} i^2 \right)
      \\
      &= \lim_{n\to\infty} \frac{3}{n} \left( -2 \sum_{i=1}^n 1 +
        \frac{12}{n} \sum_{i=1}^n i + \frac{9}{n^2} \sum_{i=1}^n i^2
        \right)
    \end{align*}
    Now we use the formulas
    \begin{equation*}
      \sum_{i=1}^n 1 = n \qquad \sum_{i=1}^n i = \frac{n(n+1)}{2}
      \qquad \sum_{i=1}^n i^2 = \frac{n(n+1)(2n+1)}{6}
    \end{equation*}
    to obtain
    \begin{align*}
      \int_1^4 (x^2 + 2x - 5) \; dx
      &= \lim_{n\to\infty} \frac{3}{n} \left( -2 n + \frac{12}{n}\cdot
        \frac{n(n+1)}{2} + \frac{9}{n^2} \cdot \frac{n(n+1)(2n+1)}{6}
        \right)
      \\
      &= \lim_{n\to\infty} \left( -6 + \frac{36}{2}\cdot \frac{n^2+n}{n^2} +
        \frac{27}{6} \cdot \frac{2n^3+3n^2+n}{n^3} \right)
      \\
      &= \lim_{n\to\infty} -6 + \lim_{n\to\infty} 18 \cdot \frac{1+1/n}{1} +
        \lim_{n\to\infty} \frac{9}{2} \cdot \frac{2 + 3/n + 1/n^2}{1}
      \\
      &= -6 + 18 \cdot \frac{1+0}{1} + \frac{9}{2} \cdot \frac{2+0+0}{1}
      \\
      &= -6 + 18 + 9 = 21
    \end{align*}
  \item %$\ds \int_0^5 (1+2x^3) \; dx$
    Here we have $a=0$, $b=5$, and $f(x)=1+x^3$.  Then
    \begin{equation*}
      \Delta x = \frac{b-a}{n} = \frac{5-0}{n} = \frac{5}{n}
    \end{equation*}
    and
    \begin{equation*}
      x_i = a + i \Delta x = 0 + i \frac{5}{n} = \frac{5i}{n}
    \end{equation*}
    The integral as a limit of a Riemann sum is
    \begin{align*}
      \int_0^5 (1+2x^3) \; dx
      &= \lim_{n\to\infty} \sum_{i=1}^n (1+2x_i^3) \; \Delta x
      \\
      &= \lim_{n\to\infty} \sum_{i=1}^n \left(1 +
        2\left(\frac{5i}{n}\right)^3\right) \; \frac{5}{n}
      \\
      &= \lim_{n\to\infty} \frac{5}{n} \left(\sum_{i=1}^n 1 + 2 \cdot
        \frac{5^3}{n^3} \sum_{i=1}^n i^3 \right) 
    \end{align*}
    Now using the formulas
    \begin{equation*}
      \sum_{i=1}^n 1 = n \qquad \sum_{i=1}^n i^3 =
      \left(\frac{n(n+1)}{2}\right)^2 = \frac{n^4 + 2n^3 + n^2}{4}
    \end{equation*}
    we have
    \begin{align*}
      \int_0^5 (1+2x^3) \; dx
      &= \lim_{n\to\infty} \frac{5}{n} \left( n + \frac{250}{n^3}
        \cdot \frac{n^4+2n^3+n^2}{4} \right)
      \\
      &= \lim_{n\to\infty} \left(5 + \frac{625}{2}
        \cdot \frac{n^4+2n^3+n^2}{n^4}\right) 
      \\
      &= \lim_{n\to\infty} \left(5 + \frac{625}{2}
        \cdot \frac{1+2/n+1/n^2}{1}\right)
      \\
      &= 5 + \frac{625}{2} = \frac{635}{2}
    \end{align*}
  \end{enumerate}
\item %(Based on 4.2.44)
  %Use the properties of integrals and the result $\ds\int_2^5 x^4\; dx=618.6$
  %to evaluate $\ds\int_2^5 (1+3x^4) \; dx$.
  We have
  \begin{equation*}
    \int_2^5 (1+3x^4) \; dx = \int_2^5 1 \; dx + \int_2^5 3x^4 \; dx
    = \int_2^5 1 \; dx + 3\int_2^5 x^4 \; dx
  \end{equation*}
  by the rules for the integral of a sum and the integral of a
  constant multiple.  Now using
  \begin{equation*}
    \int_a^b c \; dx = c(b-a)
  \end{equation*}
  and the given information we have
  \begin{equation*}
    \int_2^5 (1+3x^4) \; dx = 1(5-2) + 3(618.6) = 3 + 1855.8 = 1858.8
  \end{equation*}
\item %(Based on 4.2.30)
  %Express the integral $\ds \int_0^{2\pi} x^2 \sin x \; dx$
  %as a limit of Riemann sums.  Do not evaluate.
  We have $a=0$, $b=2\pi$, so
  \begin{equation*}
    \Delta x = \frac{b-a}{n} = \frac{2\pi}{n}
    \qquad
    x_i = a + i \Delta x = \frac{2\pi i}{n}
  \end{equation*}
  Then the integral is
  \begin{equation*}
    \int_0^{2\pi} x^2 \sin x \; dx
    = \lim_{n\to\infty} \sum_{i=1}^n x_i^2 \sin(x_i) \frac{2\pi}{n}
  \end{equation*}
  You can substitute $x_i = 2\pi i/n$ in the above expression if you
  like.  The limit would be very difficult to evaluate given our
  current knowledge, but is not impossible.
\item %(Based on 4.2.18--20)
  %Express the limit as a definite integral on the given interval.
  \begin{enumerate}
  \item %$\ds\lim_{n\to\infty}\sum_{i=1}^n \frac{\cos x_i}{x_i} \Delta x$,
    % $[\pi,2\pi]$
    We have $a=\pi$, $b=2\pi$, and $\ds f(x) = \frac{\cos x}{x}$ so
    the integral is
    \begin{equation*}
      \int_{\pi}^{2\pi} \frac{\cos x}{x} \; dx
    \end{equation*}
  \item %$\ds\lim_{n\to\infty}\sum_{i=1}^n [4-3(x_i^*)^2+6(x_i^*)^5]\Delta x$,
    % $[0,2]$
    We have $a=0$, $b=2$, and $\ds f(x) =  4 - 3x^2 + 6 x^5$ so the
    integral is
    \begin{equation*}
      \int_0^2 (4-3x^2+6x^5) \; dx
    \end{equation*}
  \end{enumerate}
\item\label{sol:042:areas}%(Based on 4.2.36--40)
  %Evaluate the following integrals by interpreting them in terms of areas.
  \begin{enumerate}
  \item %$\ds\int_{-2}^2 \sqrt{4-x^2} \; dx$
    We have $y=\sqrt{4-x^2}$ which implies $y^2=4-x^2$ or $x^2+y^2=4$,
    which is the equation of a circle with center $(0,0)$ and radius
    $\sqrt{4}=2$.  Since $y=\sqrt{4-x^2}$ is the positive square root
    we take the upper half of the circle for the function we are
    integrating (see Figure~\ref{graph:042:areas}(a)).  Using the
    formula for the area of a circle, which is $\pi r^2$, the area $A$
    is the area of a semi-circle of radius $2$, which is $\pi 2^2/2 = 2\pi$.
  \item %$\ds\int_{-1}^3 (3-2x) \; dx$
    We graph the line $y=3-2x$ from $x=-1$ to $x=3$.  Note that the
    line crosses the $x$-axis, so the area $A_1$ is positive while the
    area $A_2$ is negative (see Figure~\ref{graph:042:areas}(b)).
    $A_1$ is the area of a triangle with base $3/2-(-1) = 5/2$ and
    height $5$, so is $1/2$ base $\times$ height =
    $1/2 \times 5/2 \times 5 = 25/4$.  $A_2$ is the area of a triangle
    with base $3-3/2 = 3/2$ and height $3$, so
    $A_2 = 1/2 \times 3/2 \times 3 = 9/4$.  Altogether the integral is
    the net area $A_1-A_2 = 25/4 - 9/4 = 16/4 = 4$ units.
  \item %$\ds\int_0^{10} |x-5| \; dx$
    We graph the function $y=|x-5|$ from $x=0$ to $x=10$ by breaking
    it into two cases, from $x=0$ to $x=5$ and then from $x=5$ to
    $x=10$ (see Figure~\ref{graph:042:areas}(c)).  The integral is the
    sum of two positive areas, both of which are triangles.  $A_1=1/2$
    base $\times$ height = $1/2 \times 5 \times 5 = 25/2$.  Similarly
    $A_2=25/2$.  Altogether the integral is $A_1+A_2=25/2 + 25/2 = 25$.
  \end{enumerate}
  \begin{figure}[htbp]
    \centering
    $\begin{array}{c@{\hspace{0.25in}}c@{\hspace{0.25in}}c}
        \begin{tikzpicture}[declare function={a=-2;b=2;f(\x)=sqrt(4-(\x)^2);}]
          \begin{axis}[
            axis lines=middle,
            axis equal,
            axis on top,
            width=7.0cm,
            xmin=-2.5,
            xmax=2.5,
            xlabel=$x$,
            ylabel=$y$,
            xtick={-2,-1,0,1,2},
            xticklabels={$-2$,,,,$2$},
            grid=both
            ]
            \addplot[name path=A,red,domain=-2:2,samples=300,smooth]
            {f(x)};
            \path[name path=B] (-2,0) -- (2,0);
            \addplot[red!30] fill between [
            of=A and B,
            ];
            \path (0.5,0.5) node{$A$};
          \end{axis}
       \end{tikzpicture}
       &
         \begin{tikzpicture}[declare function={f(\x)=3-2*(\x);}]
           \begin{axis}[
             axis lines=middle,
             axis on top,
             width=7.0cm,
             xmin=-1.5,
             xmax=3.5,
             ymin=-3.5,
             ymax=5.5,
             xlabel=$x$,
             ylabel=$y$,
             xtick={-1,-0.5,0,0.5,1,1.5,2,2.5,3},
             xticklabels={$-1$,,,,,$\frac{3}{2}$,,,$3$},
             ytick={-3,-2,-1,0,1,2,3,4,5},
             yticklabels={$-3$,,,,,,,,$5$},
             grid=major
             ]
             \addplot[name path=A,red,domain=-1:1.5] {f(x)};
             \path[name path=B] (-1,5) -- (-1,0) -- (1.5,0);
             \addplot[red!30] fill between [
             of=A and B, 
             ];
             \addplot[name path=C,orange,domain=1.5:3] {f(x)};
             \path[name path=D] (1.5,0) -- (3,0) -- (3,-3);
             \addplot[orange!30] fill between [
             of=C and D,
             ];
             \path (-0.25,1.5) node{$A_1$};
             \path (2.75,-1.5) node{$A_2$};
           \end{axis}
         \end{tikzpicture}
       &
         \begin{tikzpicture}[declare function={f(\x)=abs(x-5);}]
           \begin{axis}[
             axis lines=middle,
             axis on top,
             width=7.0cm,
             xmin=-0.5,
             xmax=10.5,
             ymin=-0.5,
             ymax=5.5,
             xlabel=$x$,
             ylabel=$y$,
             xtick={1,2,3,4,5,6,7,8,9,10},
             xticklabels={$1$,$2$,$3$,$4$,$5$,$6$,$7$,$8$,$9$,$10$},
             ytick={1,2,3,4,5},
             yticklabels={$1$,$2$,$3$,$4$,$5$},
             grid=major
             ]
             \addplot[name path=A,red,domain=0:10] {f(x)};
             \path[name path=B] (0,0)--(10,0);
             \addplot[red!30] fill between [
             of=A and B,soft clip={domain=0:10}
             ];
             \path (1.5,1.5) node{$A_1$};
             \path (8.5,1.5) node{$A_2$};
           \end{axis}
         \end{tikzpicture}
       \\
       \mbox{(a) $y=\sqrt{4-x^2}$}
       &
         \mbox{(b) $y=3-2x$}
       &
         \mbox{(c) $y=|x-5|$}
     \end{array}$
    \caption{Graphs for Solution~\ref{sol:042:areas}}
    \label{graph:042:areas}
  \end{figure}
\item %(Based on 4.2.28)
  % Show that $\ds \int_a^b x^2 \; dx = \frac{b^3-a^3}{3}$.
  In this case $a$ and $b$ are unspecified so we can't evaluate
  $\Delta x$ explicitly.  We must write
  \begin{equation*}
    \Delta x = \frac{b-a}{n}
  \end{equation*}
  and
  \begin{equation*}
    x_i = a + i \frac{b-a}{n} 
  \end{equation*}
  Evaluating the function $x^2$ at $x_i$,
  \begin{equation*}
    x_i^2 = \left(a + i \frac{b-a}{n}\right)^2 = a^2 +
    2ai\frac{b-a}{n} + i^2 \frac{(b-a)^2}{n^2}
  \end{equation*}
  Substituting into the formula for definite integral,
  \begin{align*}
    \int_a^b x^2 \; dx
    &= \lim_{n\to\infty} \sum_{i=1}^n x_i^2 \Delta x
    \\
    &= \lim_{n\to\infty} \sum_{i=1}^n \left(a^2 + 2ai\frac{b-a}{n} +
      i^2 \frac{(b-a)^2}{n^2}\right) \frac{b-a}{n}
    \\
    &= \lim_{n\to\infty} \left(a^2 \frac{b-a}{n} \sum_{i=1}^n 1 +
      2a\left(\frac{b-a}{n}\right)^2 \sum_{i=1}^n i +
      \left(\frac{b-a}{n}\right)^3 \sum_{i=1}^n i^2\right)
  \end{align*}
  Now using the formulas
  \begin{equation*}
    \sum_{i=1}^n 1 = n, \qquad \sum_{i=1}^n i = \frac{n^2+n}{2},
    \qquad \sum_{i=1}^n i^2 = \frac{2n^3 + 3n^2 + n}{6},
  \end{equation*}
  we have
  \begin{align*}
    \int_a^b x^2 \; dx
    &= \lim_{n\to\infty} \left(a^2 \frac{b-a}{n} n +
      2a\left(\frac{b-a}{n}\right)^2 \frac{n^2+n}{2} +
      \left(\frac{b-a}{n}\right)^3 \frac{2n^3+3n^2+n}{6} \right)
    \\
    &= a^2(b-a) + a(b-a)^2 \lim_{n\to\infty} \frac{n^2+n}{n^2} +
      (b-a)^3 \lim_{n\to\infty} \frac{2n^3 + 2n^2 + n}{6n^3}
    \\
    &= a^2(b-a) + a(b-a)^2 + \frac{1}{3} (b-a)^3
    \\
    &= a^2 b - a^3 + ab^2 - 2a^2b + a^3 + \frac{1}{3} b^3 - ab^2 +
      a^2b - \frac{1}{3} a^3
    \\
    &= \frac{b^3-a^3}{3}
  \end{align*}
  \textit{Alternate Solution:} You can simplify the above calculation
  by noting that
  \begin{equation*}
    \int_0^b x^2 \; dx = \int_0^a x^2 \; dx + \int_a^b x^2 \; dx
    \implies \int_a^b x^2 \; dx = \int_0^b x^2 \; dx - \int_0^a x^2 \;
    dx
  \end{equation*}
  so we only have to evaluate the definite integral when $0$ is the
  lower limit of integration.  In that case,
  \begin{equation*}
    \Delta x = \frac{b-0}{n} = \frac{b}{n} \qquad x_i = a + i \Delta x
    = 0 + i \frac{b}{n} = \frac{bi}{n}
  \end{equation*}
  which are simpler than in the previous solution.  Then
  \begin{align*}
    \int_0^b x^2 \; dx
    &= \lim_{n\to\infty} \sum_{i=1}^n x_i^2 \; \Delta x
     = \lim_{n\to\infty} \sum_{i=1}^n \left(\frac{bi}{n}\right)^2
      \frac{b}{n}
    = \lim_{n\to\infty} \frac{b^3}{n^3} \sum_{i=1}^n i^2
    \\
    &= \lim_{n\to\infty} \frac{b^3}{n^3} \frac{2n^3+3n^2+n}{6}
    = \lim_{n\to\infty} b^3 \frac{2n^3+3n^2+n}{6n^3}
    \\
    &= b^3 \frac{2}{6} = \frac{b^3}{3}
  \end{align*}
  Substituting $b$ with $a$ in the above calculation gives
  \begin{equation*}
    \int_0^a x^2 \; dx = \frac{a^3}{3}
  \end{equation*}
  so finally
  \begin{equation*}
    \int_a^b x^2 \; dx = \int_0^b x^2 \; dx - \int_0^a x^2 \; dx
    = \frac{b^3}{3} - \frac{a^3}{3}
  \end{equation*}
\end{enumerate}


\end{document}

