\documentclass{article}
\usepackage{amsmath}
\usepackage{fullpage}
%\usepackage{graphicx}
\usepackage{tikz}
% \allowdisplaybreaks
\usepackage[aux]{rerunfilecheck}

\newcommand{\ds}{\displaystyle}

\input{../common.tex}

\title{\commonPSTitleZeroTwoSix\ Solutions}
\author{\commonAuthor}
\date{\commonDateZeroTwoSix}

\begin{document}
\maketitle
\begin{enumerate}
\item %1
  \begin{enumerate}
  \item Differentiating both sides of the equation,
    \begin{align*}
      \frac{d}{dx} (x^2+xy-y^2) &= \frac{d}{dx} 4 \\
      \frac{d}{dx} x^2 + \frac{d}{dx} xy - \frac{d}{dx} y^2 &= 0 \\
    \end{align*}
    We apply the power rule to the first term, the product rule to the
    second, and the power-chain rule to the third:
    \begin{align*}
      2x + \left( \frac{d}{dx} x\right) y + x \left(\frac{d}{dx}
      y\right) - 2y \frac{d}{dx} y &= 0 \\
      2x + y + x \frac{dy}{dx} - 2y \frac{dy}{dx} &= 0
    \end{align*}
    Solving for $dy/dx$,
    \begin{align*}
      x \frac{dy}{dx} - 2y \frac{dy}{dx} &= -2x - y \\
      (x-2y) \frac{dy}{dx} &= -2x-y \\
      \frac{dy}{dx} &= \frac{-2x-y}{x-2y}
    \end{align*}
  \item Write the roots in terms of powers and differentiate both
    sides of the equation:
    \begin{align*}
      x^{1/2} + 2y^{1/2} &= 3 \\
      \frac{d}{dx} (x^{1/2} + 2y^{1/2}) &= \frac{d}{dx} 3 \\
      \frac{d}{dx} x^{1/2} + 2\frac{d}{dx} y^{1/2} &= 0
    \end{align*}
    By the power rule and the power-chain rule,
    \begin{align*}
      \frac{1}{2} x^{-1/2} + 2 \frac{1}{2} y^{-1/2} \frac{dy}{dx} =0
    \end{align*}
    Solving for $dy/dx$,
    \begin{align*}
      y^{-1/2} \frac{dy}{dx} &= -\frac{x^{-1/2}}{2} \\
      \frac{dy}{dx} &= -\frac{x^{-1/2}}{2y^{-1/2}}
    \end{align*}
    The following simplification is nice but not necessary:
    \begin{align*}
      \frac{dy}{dx} &= -\frac{y^{1/2}}{2x^{1/2}} \\
      \frac{dy}{dx} &= -\frac{\sqrt{y}}{2\sqrt{x}}
    \end{align*}
  %\item Differentiating both sides of the equation,
  %  \begin{align*}
  %    \frac{d}{dx} e^{xy} &= \frac{d}{dx} (x+y) \\
  %    \frac{d}{dx} e^{xy} &= 1 + \frac{dy}{dx}
  %  \end{align*}
  %  Differentiating the left hand side by the chain rule,
  %  \begin{align*}
  %    e^{xy} \frac{d}{dx} (xy) &= 1 + \frac{dy}{dx} \\
  %    e^{xy} \left( \frac{dx}{dx} y + x \frac{dy}{dx}\right) &= 1 +
  %    \frac{dy}{dx} \\
  %    e^{xy} \left(y + x\frac{dy}{dx}\right) &= 1 + \frac{dy}{dx} 
  %  \end{align*}
  %  Expanding,
  %  \begin{align*}
  %    ye^{xy} + xe^{xy} \frac{dy}{dx} &= 1 + \frac{dy}{dx}
  %  \end{align*}
  %  Solving for $dy/dx$,
  %  \begin{align*}
  %    xe^{xy} \frac{dy}{dx} - \frac{dy}{dx} &= 1 - ye^{xy} \\
  %    (xe^{xy} - 1) \frac{dy}{dx} &= 1-ye^{xy} \\
  %    \frac{dy}{dx} &= \frac{1-ye^{xy}}{xe^{xy}-1}
  %  \end{align*}
  \item Differentiating both sides,
    \begin{align*}
      \frac{d}{dx} \left(x^3(x-y)\right) &= \frac{d}{dx}
      \left(y^2(x+3y)\right) \\
      \left(\frac{d}{dx} x^3\right) (x-y) + x^3
      \left(\frac{d}{dx}(x-y)\right) &= \left(\frac{d}{dx} y^2 \right)
      (x+3y) + y^2 \left( \frac{d}{dx} (x+3y) \right) 
    \end{align*}
    where we have used the product rule.  By the power rule,
    difference rule, power-chain rule, and sum rule,
    \begin{align*}
      3x^2 (x-y) + x^3 \left(1-\frac{dy}{dx}\right) &= 2y
      \frac{dy}{dx} (x+3y) + y^2 \left( 1+3\frac{dy}{dx} \right)
    \end{align*}
    Solving for $dy/dx$,
    \begin{align*}
      3x^2(x-y) + x^3 - x^3 \frac{dy}{dx} &= 2y(x+3y) \frac{dy}{dx} +
      y^2 + 3y^2 \frac{dy}{dx} \\
      (-x^3 - 2xy - 6y^2 - 3y^2) \frac{dy}{dx} &= y^2 - 3x^3 + 3x^2y -
      x^3 \\
      \frac{dy}{dx} &= \frac{-4x^3 + y^2 + 3x^2y}{-x^3-2xy-9y^2}
    \end{align*}
  \end{enumerate}
\item %2
  \begin{enumerate}
  \item Differentiating both sides,
    \begin{equation*}
      2x + y + x\frac{dy}{dx} + 2y \frac{dy}{dx} = 0
    \end{equation*}
    Solving for $dy/dx$,
    \begin{equation*}
      (x+2y) \frac{dy}{dx} = -2x-y \implies \frac{dy}{dx} =
      \frac{-2x-y}{x+2y}
    \end{equation*}
    At the point $(x,y)=(1,2)$ we have 
    \begin{equation*}
      \frac{dy}{dx} = \frac{-2x-y}{x+2y} = \frac{-2(1)-(2)}{(1)+2(2)}
      = \frac{-4}{5}
    \end{equation*}
    The slope of the tangent line is $-4/5$, so the equation of the
    tangent line is
    \begin{equation*}
      y-y_0 = m(x-x_0) \implies y-2 = -\frac{4}{5} (x-1)
    \end{equation*}
  \item Differentiating both sides,
    \begin{equation*}
      \frac{2}{3} x^{-1/3} + \frac{2}{3} y^{-1/3} \frac{dy}{dx} = 0
      \implies x^{-1/3} + y^{-1/3} \frac{dy}{dx} = 0
    \end{equation*}
    Solving for $dy/dx$,
    \begin{equation*}
      y^{-1/3} \frac{dy}{dx} = -x^{-1/3}
      \implies \frac{dy}{dx} = -\frac{x^{-1/3}}{y^{-1/3}} =
      -\left(\frac{y}{x}\right)^{1/3} 
    \end{equation*}
    At the point $\ds \left(-\frac{64}{27},-1\right)$ we have
    \begin{equation*}
      \frac{dy}{dx} = -\left(\frac{y}{x}\right)^{1/3} =
      -\left(\frac{-64/27}{-1}\right)^{1/3} =
      -\left(\frac{64}{27}\right)^{1/3} = -\frac{4}{3}
    \end{equation*}
    So an equation for the tangent line is
    \begin{equation*}
      y+1 = -\frac{4}{3} \left(x+\frac{64}{27}\right)
    \end{equation*}
  \end{enumerate}
\item %3
  Differentiating both sides,
  \begin{align*}
    \frac{d}{dx} 2(x^2+y^2)^2 &= \frac{d}{dx} 25(x^2-y^2) \\
    2 \frac{d}{dx} (x^2+y^2)^2 &= 25 \frac{d}{dx} (x^2-y^2)
  \end{align*}
  By the chain rule we have
  \begin{align*}
    2 \cdot 2(x^2+y^2) \cdot \frac{d}{dx}(x^2+y^2) &= 25 \frac{d}{dx} (x^2-y^2) 
  \end{align*}
  By the sum and difference rules, the power rule, and the power-chain rule,
  \begin{align*}
    4(x^2+y^2) \left(2x + 2y \frac{dy}{dx}\right)
    &= 25 \left(2x-2y \frac{dy}{dx}\right)
  \end{align*}
  Expanding and gathering,
  \begin{align*}
    8x(x^2+y^2) + 8y(x^2+y^2) \frac{dy}{dx} &= 50 x - 50 y \frac{dy}{dx} \\
    8y(x^2+y^2) \frac{dy}{dx} + 50y\frac{dy}{dx} &= 50x - 8x(x^2+y^2) \\
    \frac{dy}{dx} &= \frac{50x-8x(x^2+y^2)}{8y(x^2+y^2) + 50y}
  \end{align*}
  At the point $(x,y)=(3,-1)$ we have
  \begin{align*}
    \frac{dy}{dx} &= \frac{50(3)-8(3)(3^2+(-1)^2)}{8(-1)(3^2+(-1)^2)+50(-1)} \\
                  &= \frac{150 - 24(9+1)}{-8(9+1)-50}
                    = \frac{150-240}{-80-50} = \frac{-90}{-130} \\
                  &= \frac{9}{13}
  \end{align*}
  It follows that the equation of the tangent line is
  \begin{equation*}
    y-y_0 = m (x-x_0) \implies y+1 = \frac{9}{13}(x-3) 
  \end{equation*}
  and the equation of the normal line is
  \begin{equation*}
    y-y_0 = -\frac{1}{m} (x-x_0) \implies y+1 = -\frac{13}{9} (x-3)
  \end{equation*}
\item %4
  \begin{enumerate}
  \item Differentiating both sides,
    \begin{equation*}
      8x + 18yy' = 0 \implies 9yy' = -4x \implies y' = -\frac{4x}{9y}
    \end{equation*}
    Differentiating again,
    \begin{equation*}
      y'' = -\frac{4(9y) - 4x(9y')}{y^2} = -\frac{36y - 36xy'}{y^2}
    \end{equation*}
    Substituting $y'$ from above,
    \begin{equation*}
      y'' = -\frac{36y-36x\left(-\frac{4x}{9y}\right)}{y^2}
    \end{equation*}
    Further simplification is nice, but is not necessary:
    \begin{equation*}
      y'' = -\frac{36y + 16 \frac{x}{y}}{y^2} 
      = -\frac{36y^2+16x^2}{y^3} = -\frac{4(9y^2+4x^2)}{y^3} 
      = -\frac{4(36)}{y^3}
    \end{equation*}
    where we have used the equation $4x^2+9y^2=36$ to simplify the
    above expression.  
  \item (Note that $a$ is a constant.)  Differentiating both sides,
    \begin{equation*}
      3x^2 + 3y^2y' = 0 \implies y' = -\frac{x^2}{y^2}
    \end{equation*}
    Differentiating again by the quotient rule,
    \begin{equation*}
      y'' = -\frac{2xy^2 - x^2\cdot 2yy'}{y^4}
    \end{equation*}
    Substituting $y'$ from above,
    \begin{equation*}
      y'' = -\frac{2xy^2-2x^2yy'}{y^4} =
      -\frac{2xy^2-2x^2y\left(-\frac{x^2}{y^2}\right)}{y^4}
    \end{equation*}
    Further simplification is possible (but not necessary).
    Multiplying through by $y^2$ to clear fractions,
    \begin{equation*}
      y'' = -\frac{2xy^4 - 2x^2y (-x^2)}{y^6}
      = -\frac{2xy(y^3+x^3)}{y^6} = -\frac{2xa^3}{y^5}
    \end{equation*}
    where we have used $x^3+y^3=a^3$ to simplify.
  \end{enumerate}
\item %5 % EJD: Solution is wrong?  Should move function to other side and
  % get rid of inverse functions, then differentiate
  For this problem, we need the results
  \begin{equation*}
    \mbox{$\ds (\sin^{-1})' (u) = \frac{1}{\sqrt{1-u^2}}$ and
      $\ds (\tan^{-1})' (u) = \frac{1}{1+u^2}$}
  \end{equation*}
  \begin{enumerate}
  \item By the chain rule,
    \begin{equation*}
      \frac{d}{dx} \sin^{-1}\sqrt{x} = (\sin^{-1})' (\sqrt{x}) \cdot
      \frac{d}{dx} \sqrt{x}
      = \frac{1}{\sqrt{1-(\sqrt{x})^2}} \cdot \frac{1}{2\sqrt{x}}
      = \frac{1}{2\sqrt{x}\sqrt{1-x}}
    \end{equation*}
  \item By the chain rule
    \begin{equation*}
      \frac{d}{dx} \sqrt{\sin^{-1}(x)}
      = \frac{1}{2} (\sin^{-1}(x))^{-1/2} \cdot \frac{1}{\sqrt{1-x^2}}
    \end{equation*}
  \item By the chain rule applied to the term $\tan^{-1}(1/t) =
    \tan^{-1}(t^{-1})$, 
    \begin{equation*}
      y' = \frac{1}{1+t^2} + \frac{1}{1+(1/t)^2} \cdot (-1)t^{-2}
      = \frac{1}{1+t^2} -\frac{1}{t^2+1} = 0
    \end{equation*}
  \item By the chain rule,
    \begin{equation*}
      f'(\theta) 
      = \frac{1}{\sqrt{1-(2\sin\theta)^2}} \cdot 2\cos \theta
    \end{equation*}
  \end{enumerate}
\item %6 EJD: this is easy, move earlier
  Differentiating by the chain and product rules,
  \begin{equation*}
    2f(x)f'(x) + f(x) + xf'(x) = 0
  \end{equation*}
  Solving for $f'(x)$,
  \begin{equation*}
    (2f(x)+x)f'(x) = -f(x) \implies f'(x) = -\frac{f(x)}{2f(x)+x}
  \end{equation*}
  Substituting $x=2$,
  \begin{equation*}
    f'(2) = -\frac{f(2)}{2f(2)+2}
  \end{equation*}
  Substituting $f(2)=1$,
  \begin{equation*}
    f'(2) = -\frac{1}{2(1)+2} = -\frac{1}{4}
  \end{equation*}
\item %7
  Differentiating by $d/dy$,
  \begin{align*}
    \frac{d}{dy} (x^3y^2) - \frac{d}{dy} (xy^3) + 3\frac{d}{dy}(xy) &=
    0
  \end{align*}
  By the product rule,
  \begin{align*}
    \frac{d}{dy} x^3 \cdot y^2 + x^3 \frac{d}{dy} y^2
    - \frac{d}{dy} x \cdot y^3 - x\frac{d}{dy} y^3 
    + 3\frac{d}{dy} x \cdot y + 3x \frac{d}{dy} y = 0
  \end{align*}
  Since $x$ is dependent on $y$, the chain rule says
  \begin{equation*}
    \frac{d}{dy} x^3 = 3x^2 \frac{dx}{dy}
  \end{equation*}
  etc., so we have
  \begin{equation*}
    3x^2y^2 \frac{dx}{dy} + 2x^3 y - y^3 \frac{dx}{dy} - 3xy^2 +
    3y\frac{dx}{dy} + 3x = 0
  \end{equation*}
  Solving for $dx/dy$,
  \begin{equation*}
    (3x^2y^2-y^3+3y) \frac{dx}{dy} = -3x^3y+3xy^2-3x 
    \implies \frac{dx}{dy} = \frac{-3x^3y+3xy^2-3x}{3x^2y^2-y^3+3y}
  \end{equation*}
  You might compare with the result of finding $dy/dx$.  How are the
  two results related?
\item %8 EJD: this works better with tangent line; try tangent to hyperbola
  Differentiating with respect to $x$,
  \begin{equation*}
    \frac{2x}{a^2} + \frac{2yy'}{b^2} = 0
  \end{equation*}
  Solving for $y'$,
  \begin{equation*}
    \frac{yy'}{b^2} = -\frac{x}{a^2} \implies y' = -\frac{b^2x}{a^2y}
  \end{equation*}
  At a point $(x_0,y_0)$ on the ellipse, the slope of the tangent line
  is
  \begin{equation*}
    y' = -\frac{b^2x_0}{a^2y_0}
  \end{equation*}
  and the slope of the normal line is therefore the negative reciprocal
  \begin{equation*}
    -\frac{1}{y'} = \frac{a^2y_0}{b^2x_0}
  \end{equation*}
  An equation of the normal line is therefore
  \begin{equation*}
    y-y_0 = \frac{a^2y_0}{b^2x_0} (x-x_0)
  \end{equation*}
\item %9
  The slope of the tangent at $(x,y)$ to one of the parabolas is found by
  \begin{equation*}
    1 = 2cyy' \implies y_p' = \frac{1}{2cy}
  \end{equation*}
  The slope of the tangent at $(x,y)$ to one of the ellipses is found
  by
  \begin{equation*}
    4x + 2yy' = 0 \implies y_e' = -\frac{2x}{y}
  \end{equation*}
  The product of the two slopes is
  \begin{equation*}
    y_p' y_e' = \frac{1}{2cy} \cdot -\frac{2x}{y} = -\frac{x}{cy^2} 
  \end{equation*}
  Since the point $(x,y)$ lies on the parabola $x=cy^2$ we have
  $cy^2=x$ so
  \begin{equation*}
    y_p' y_e' = -\frac{x}{cy^2} = -\frac{x}{x} = -1
  \end{equation*}
  Therefore $y_e'$ is the negative reciprocal of $y_p'$, i.e., the
  tangents to the two curves are perpendicular.
\item %10
  First we find an equation of a tangent line through an arbitrary
  point $(x_0,y_0)$ on the ellipse.  Differentiating,
  \begin{equation*}
    \frac{2x}{3^2} + \frac{2yy'}{6^2} = 0
    \implies 
    \frac{yy'}{6^2} = -\frac{x}{3^2}
    \implies 
    y' = -\frac{6^2x}{3^2y} = -\frac{4x}{y}
  \end{equation*}
  So an equation of the tangent line at $(x_0,y_0)$ is
  \begin{equation*}
    y-y_0 = -\frac{4x_0}{y_0} (x-x_0)
    \implies
    y_0y - y_0^2 + 4x_0 x - 4x_0^2 = 0
    \implies 4x_0x + y_0y = 4x_0^2 + y_0^2 = 36
  \end{equation*}
  (the latter equality is a consequence of $(x_0,y_0)$ being on the
  ellipse).  Since the tangent line also passes through $(3,12)$, the
  point $(x,y)=(3,12)$ satisfies the equation of the tangent line,
  i.e.,
  \begin{equation*}
    12x_0 + 12y_0 = 36
  \end{equation*}
  We therefore have a system of equations for $(x_0,y_0)$:
  \begin{align*}
    4x_0^2 + y_0^2 &= 36 \\
    12x_0 + 12y_0 &= 36
  \end{align*}
  Solving the second equation for $y_0$,
  \begin{equation*}
    y_0 = 3 - x_0
  \end{equation*}
  Substituting that into the first equation,
  \begin{equation*}
    4x_0^2 + y_0^2 = 36
    \implies 4x_0^2 + (3-x_0)^2 = 36
  \end{equation*}
  Expanding and gathering,
  \begin{equation*}
    4x_0^2 + 9 - 6x_0 + x_0^2 = 36
    \implies 5x_0^2 - 6x_0 - 27 = 0
  \end{equation*}
  The equation factors as
  \begin{equation*}
    (5x_0+9)(x_0-3)=0 \implies x=-\frac{9}{5} \quad\mbox{or}\quad x=3
  \end{equation*}
  The corresponding $y_0$ values are respectively $y_0=3+(9/5)=24/5$
  and $y_0=3-3=0$.  So the two lines are
  \begin{align*}
    \frac{24}{5} y - \frac{24^2}{5^2} - 4\frac{9}{5} x - 4\frac{9^2}{5^2} &= 0
    \\
    0 y - 0 - 4(3) x - 4(3^2) &= 0
  \end{align*}
  You can simplify the equations of the lines.
  % EJD: check with graph
  % EJD: change to hyperbola problem and use hyperbola version of
  % problem 8 (with particular numbers a, b
\end{enumerate}
\end{document}
