\documentclass{article}
\usepackage{fullpage}
\usepackage{amsmath}
\usepackage{multicol}
\usepackage{mathptmx}

\newcommand{\ds}{\displaystyle}

\input{../common.tex}

\title{\commonPSTitleZeroFourFive\ Solutions}
\author{\commonAuthor}
\date{\commonDateZeroFourFive}

\begin{document}
\maketitle
\begin{enumerate}
\item
  \begin{enumerate}
  \item Let $u=x^3+5$.  Then $du/dx = 3x^2$, $du/3 = x^2 \; dx$ and
    \begin{equation*}
      \int x^2(x^3+5)^9 \; dx = \int u^9 \frac{du}{3} = \frac{1}{30} u^{10} + C
      = \frac{1}{30} (x^3+5)^{10} + C
    \end{equation*}
    Check by differentiating.
  \item Let $u=3t+2$.  Then $du/dt = 3$, $du/3 = dt$ and
    \begin{equation*}
      \int (3t+2)^{2.4} \; dt = \int u^{2.4} \; \frac{du}{3}
      = \frac{1}{3} \int u^{2.4} \; du = \frac{1}{3}
      \frac{u^{3.4}}{3.4} + C = \frac{1}{10.2} (3t+2)^{3.4} + C
    \end{equation*}
    Check by differentiating.
  \item Let $u=x^2+1$.  Then $du/dx = 2x$, $du/2 = x\; dx$ and
    \begin{equation*}
      \int \frac{x}{(x^2+1)^2} \; dx = \int u^{-2} \frac{du}{2}
      = -\frac{1}{2} u^{-1} + C = -\frac{1}{2(x^2+1)} + C
    \end{equation*}
    Check by differentiating.
  \item Let $u=5t+4$, $du/dt = 5$, $du/5 = dt$.  Then
    \begin{equation*}
      \int \frac{1}{(5t+4)^{2.7}} \; dt
      = \int u^{-2.7} \frac{du}{5}
      = \frac{1}{5} \frac{u^{-1.7}}{-1.7} + C
      = -\frac{1}{8.5} (5t+4)^{-1.7} + C
    \end{equation*}
    Check by differentiating.
  \end{enumerate}
\item
  \begin{enumerate}
  \item Let $u=2\theta$, $du=2\; d\theta$, $du/2 = d\theta$:
    \begin{equation*}
      \int \sec 2\theta \tan 2\theta \; d\theta
      = \int \sec u \tan u \; \frac{du}{2}
      = \frac{1}{2} \sec u + C
      = \frac{1}{2} \sec 2\theta + C
    \end{equation*}
    Check by differentiating.
  \item Let $u=1+x^{3/2}$.  Then $du/dx = 3x^{1/2}/2$, $2\; du/3 =
    \sqrt{x} \; dx$ and
    \begin{equation*}
      \int \sqrt{x} \sin(1+x^{3/2} \; dx
      = \frac{2}{3} \int \sin u \; du
      = -\frac{2}{3} \cos u + C
      = -\frac{2}{3} \cos (1+x^{3/2}) + C
    \end{equation*}
    Check by differentiating.
  \item Let $u=\pi/x$, $du/dx = -\pi/x^2$, $-du/\pi = dx/x^2$.  Then
    \begin{equation*}
      \int \frac{\cos(\pi/x)}{x^2} \; dx
      = -\frac{1}{\pi} \int \cos u \; du
      = -\frac{1}{\pi} \sin u + C
      = -\frac{1}{\pi} \sin(\pi/x) + C
    \end{equation*}
    Check by differentiating.
  \item Let $u=1+\tan\theta$, $du/d\theta = \sec^2\theta$, $du =
    \sec^2\theta d\theta$.  Then
    \begin{equation*}
      \int (1+\tan\theta)^5 \sec^2\theta \; d\theta
      = \int u^5 \; du
      = \frac{1}{6} u^6 + C
      = \frac{1}{6} (1+\tan\theta)^6 + C
    \end{equation*}
    Check by differentiating.
  \end{enumerate}
\item These ones are a little trickier than the previous.
  \begin{enumerate}
  \item Let $u=1+\tan t$, $du/dt = \sec^2 t$, $du = \sec^2 t \; dt =
    dt/\cos^2 t$ where we have used the trig identity $\sec^2 t =
    1/\cos^2 t$.  Then
    \begin{equation*}
      \int \frac{dt}{\cos^2t \sqrt{1+\tan t}}
      = \int u^{-1/2} \; du
      = 2 u^{1/2} + C
      = 2 \sqrt{1+\tan t} + C
    \end{equation*}
    Check by differentiating.
  \item Let $u=\cos t$, $du/dt = -\sin t$, $-du = \sin t\; dt$.  Then
    \begin{equation*}
      \int \sin t \sec^2(\cos t) \; dt
      = -\int \sec^2 u \; du
      = -\sec u + C
      = -\sec(\cos t) + C
    \end{equation*}
  \item Let $u=1-x$, $du = -dx$, $-du = dx$.  Then
    \begin{equation*}
      \int \frac{x^2}{\sqrt{1-x}} \; dx
      = -\int \frac{x^2}{\sqrt{u}} \; du
    \end{equation*}
    Unfortunately, that substitution is not complete, because not all
    of the $x$s have been eliminated from the integral.  In order to
    complete the substitution we need to go back to $u=1-x$ and solve
    for $x$: $x=1-u$.  So we can write
    \begin{equation*}
      -\int \frac{x^2}{\sqrt{u}} \; du
      = -\int \frac{(1-u)^2}{u^{1/2}} \; du
      = -\int \frac{1-2u+u^2}{u^{1/2}} \; du
      = -\int (u^{-1/2} - 2 u^{1/2} + u^{3/2}) \; du
    \end{equation*}
    Integrating by the power rule we have
    \begin{equation*}
      \int \frac{x^2}{\sqrt{1-x}} \; dx
      = -2u^{1/2} - \frac{4}{3} u^{3/2} + \frac{2}{5} u^{5/2} + C
      = -2(1-x)^{1/2} - \frac{4}{3} (1-x)^{3/2} + \frac{2}{5}
      (1-x)^{5/2} + C
    \end{equation*}
    You should check your answer by differentiating, then doing some
    algebra. 
  \item Let $u=x^2+1$, $du/dx = 2x$, $du/2 = x\; dx$.  Then
    \begin{equation*}
      \int x^3 \sqrt{x^2+1} \; dx
      = \frac{1}{2} \int x^2 \sqrt{u} \; du
    \end{equation*}
    Again, the substitution hasn't been completed.  We must eliminate
    $x^2$: $u=x^2+1$ gives $x^2 =u-1$ so
    \begin{equation*}
      \frac{1}{2} \int x^2 \sqrt{u} \; du = \frac{1}{2} \int (u-1)^2
      u^{1/2} \; du
      = \frac{1}{2} \int (u^2-2u+1)u^{1/2} \; du
      = \frac{1}{2} \int (u^{5/2} - 2u^{3/2} + u^{1/2}) \; du
    \end{equation*}
    Integrating by the power rule,
    \begin{equation*}
      \int x^3 \sqrt{x^2+1} \; dx
      = \frac{1}{7} u^{7/2} - \frac{2}{5} u^{5/2}  + \frac{1}{3}
      u^{3/2} +C
      = \frac{1}{7} (x^2+1)^{7/2} - \frac{2}{5} (x^2+1)^{5/2} +
      \frac{1}{3} (x^2+1)^{3/2} + C
    \end{equation*}
    You should check your answer by differentiating, then doing some
    algebra. 
  \end{enumerate}
\item
  \begin{enumerate}
  \item To evaluate the indefinite integral, let $u=\sin x$.  Then
    $du/dx = \cos x$, $du = \cos x \; dx$:
    \begin{equation*}
      \int \cos x \; \sin(\sin x) \; dx
      = \int \sin u \; du
      = -\cos u + C
      = -\cos(\sin x) + C
    \end{equation*}
    You should check the indefinite integral by differentiating. 
    Now by the Fundamental Theorem of Calculus,
    \begin{equation*}
      \int_0^{\pi/2} \cos x \; \sin(\sin x) \; dx
      = \left. \vphantom{\int} -\cos(\sin x) \right|_0^{\pi/2}
      = -\cos(\sin(\pi/2)) + \cos(\sin(0))
      = -\cos(1) + \cos(0) = 1 - \cos(1)
    \end{equation*}
    \emph{Alternate Solution:} We can combine the two steps above into
    one step by substituting the lower and upper bounds of integration
    when we do the substitution.  When $x=0$, $u=\sin x = \sin 0 = 0$,
    so that becomes the lower bound of integration after the
    substitution.  Similarly when $x=\pi/2$,
    $u=\sin x = \sin(\pi/2) = 1$.  The calculation becomes
    \begin{equation*}
      \int_0^{\pi/2} \cos x \; \sin(\sin x) \; dx
      = \int_0^1 \sin u \; du
      = \left. \vphantom{\int} -\cos u \right|_0^1
      = -\cos 1 + \cos 0 = 1 - \cos 1
    \end{equation*}
    That is the same answer as before, but the calculation is somewhat
    shorter because we don't have to reverse the subsitition after the
    integration step.  On the other hand, it gives you less
    opportunity to check your work by differentiating.
  \item In this problem $a$ is a constant parameter.  To evaluate the
    indefinite integral we make the substitution $u=a^2-x^2$, $du/dx =
    -2x$, $-du/2 = x \; dx$:
    \begin{equation*}
      \int x \sqrt{a^2-x^2} \; dx
      = -\frac{1}{2} \int u^{1/2} \; du
      = -\frac{1}{3} u^{3/2} + C
      = -\frac{1}{3} (a^2-x^2)^{3/2} + C
    \end{equation*}
    You can check the answer by differentiating.
    The definite integral is
    \begin{equation*}
      \int_0^a x \; \sqrt{a^2-x^2} \; dx
      = \left. \vphantom{\int} -\frac{1}{3} (a^2-x^2)^{3/2}
      \right|_0^a
      = -\frac{1}{3} (a^2-a^2)^{3/2} + \frac{1}{3} (a^2-0)^{3/2}
      = \frac{1}{3} a^3
    \end{equation*}
    \emph{Alternate Solution:} When $x=0$, $u=a^2-x^2=a^2-0=a^2$, so
    that becomes the lower bound of integration after the
    substitution.  Similarly, when $x=a$, $u=a^2-a^2 = 0$, so that
    becomes the upper bound of integration after the substition.  We
    can write
    \begin{equation*}
      \int_0^a x \; \sqrt{a^2-x^2} \; dx
      = -\frac{1}{2} \int_{a^2}^0 u^{1/2} \; du
      = -\frac{1}{2} \left. \vphantom{\int} \frac{2}{3} u^{3/2}
      \right|_{a^2}^0
      = -\frac{1}{3} (0^{3/2} - (a^2)^{3/2})
      = \frac{1}{3} a^3
    \end{equation*}
    Again, the alternate solution is shorter, but we can't check the
    indefinite integral by differentiating.
  \item Let $u=1+2x$, $du/dx = 2$, $du/2=dx$, $x=(u-1)/2$:
    \begin{equation*}
      \int \frac{x}{\sqrt{1+2x}} \; dx
      = \int \frac{(u-1)/2}{\sqrt{u}} \; \frac{du}{2}
      = \frac{1}{4} \int (u^{1/2} - u^{-1/2}) \; du
      = \frac{1}{6} u^{3/2} - \frac{1}{2} u^{1/2} + C
      = \frac{1}{6} (1+2x)^{3/2} - \frac{1}{2} (1+2x)^{1/2} + C
    \end{equation*}
    Check by differentiating and then doing some algebra.
    Now we can evaluate the definite integral:
    \begin{equation*}
      \int_0^4 \frac{x}{\sqrt{1+2x}} \; dx
      = \left. \vphantom{\int} \frac{1}{6} (1+2x)^{3/2} - \frac{1}{2}
        (1+2x)^{1/2} \right|_0^4
      = \frac{1}{6} 9^{3/2} - \frac{1}{2} 9^{1/2} - \frac{1}{6}
      1^{3/2} + \frac{1}{2} 1^{1/2}
      = \frac{27}{6} - \frac{3}{2} - \frac{1}{6} + \frac{1}{2}
      = \frac{10}{3}
    \end{equation*}
    \emph{Alternate Solution:} When $x=0$, $u=1+2x=1$, and when $x=4$,
    $u=1+2x = 9$:
    \begin{equation*}
      \int_0^4 \frac{x}{\sqrt{1+2x}} \; dx
      = \frac{1}{4} \int_1^9 (u^{1/2}-u^{-1/2}) \; du
      = \frac{1}{4} \left. \vphantom{\int} \frac{2}{3} u^{3/2} - 2
        u^{1/2} \right|_1^9
      = \frac{1}{6} 9^{3/2} - \frac{1}{2} 9^{1/2}
      - \frac{1}{6} 1^{3/2} + \frac{1}{2} 1^{1/2}
      = \frac{10}{3}
    \end{equation*}
    As usual, the alternate solution is shorter but has the
    disadvantage that you can't check the integral by differentiating.
  \item In this problem $T$ and $\alpha$ are constant parameters.  Let
    $u=2\pi t/T-\alpha$.  Then $du/dt = 2\pi/T$ and $T/(2\pi) du =
    dt$.  The indefinite integral is
    \begin{equation*}
      \int \sin(2\pi t/T-\alpha) \; dt
      = \frac{T}{2\pi} \int \sin u \; du
      = \frac{T}{2\pi} (-\cos u) + C
      = -\frac{T}{2\pi} \cos (2\pi t/T - \alpha) + C
    \end{equation*}
    which you can check by differentiating.
    Now the definite integral is
    \begin{multline*}
      \int_0^{T/2} \sin(2\pi t/T - \alpha) \; dt
      = \left. \vphantom{\int} -\frac{T}{2\pi} \cos (2\pi t/T -
        \alpha) \right|_0^{T/2}
      \\
      = -\frac{T}{2\pi} \cos (2\pi (T/2)/T - \alpha)
      +\frac{T}{2\pi} \cos (2\pi (0)/T - \alpha)
      = -\frac{T}{2\pi} \left(\cos (\pi-\alpha) - \cos(-\alpha)\right)
    \end{multline*}
    \emph{Alternate Solution:} When $t=0$, $u=2\pi
    (0)/T-\alpha=-\alpha$, and when $t=T/2$, $u=2\pi (T/2) / T -
    \alpha = \pi-\alpha$, so
    \begin{equation*}
      \int_0^{T/2} \sin(2\pi t/T - \alpha) \; dt
      =\frac{T}{2\pi} \int_{-\alpha}^{\pi-\alpha} \sin u \; du
      = \left. \vphantom{\int} -\frac{T}{2\pi} \cos u
      \right|_{-\alpha}^{\pi-\alpha}
      = -\frac{T}{2\pi} \left(\cos(\pi-\alpha) - \cos(-\alpha) \right)
    \end{equation*}
    As usual, the alternate solution is shorter, but you can't check
    the substitution by differentiating.
  \end{enumerate}
\item
  \begin{enumerate}
  \item We have
    \begin{equation*}
      \int_{-2}^2 (x+3) \sqrt{4-x^2}
      = \int_{-2}^2 \left( x\sqrt{4-x^2} + 3 \sqrt{4-x^2} \right) \;
      dx
      = \int_{-2}^2 x\sqrt{4-x^2} \; dx + 3 \int_{-2}^2 \sqrt{4-x^2}
      \; dx
    \end{equation*}
    by the rules for definite integrals.  The first integral we can do
    by the substitution $u=4-x^2$, $du/dx = -2x$, $-du/2 = x \; dx$:
    \begin{equation*}
      \int x \; \sqrt{4-x^2} \; dx
      = -\frac{1}{2} \int u^{1/2} \; du
      = -\frac{1}{3} u^{3/2} + C
      = -\frac{1}{3} (4-x^2)^{3/2} + C
    \end{equation*}
    which you should check by differentiating.  The definite integral
    is then
    \begin{equation*}
      \int_{-2}^2 x \; \sqrt{4-x^2} \; dx
      = \left. \vphantom{\int} -\frac{1}{3} (4-x^2)^{3/2}
      \right|_{-2}^2
      = -\frac{1}{3}(4-(-2)^2)^{3/2} + \frac{1}{3} (4-2^2)^{3/2}
      = 0
    \end{equation*}
    On the other hand, the second integral
    \begin{equation*}
      3\int_{-2}^2 \sqrt{4-x^2} \; dx
    \end{equation*}
    cannot be done by a substitution (at least none that you have
    learned in MATH 110; if you take MATH 111, you will learn a clever
    substitution that will work).  However, you can evaluate that
    definite integral geometrically; $y=\sqrt{4-x^2}$ is the upper
    half of a circle of radius $2$ centered at the origin $(0,0)$, so
    the integral is the area of a semicircle of radius $2$, namely
    $2\pi$.  % EJD: Graph
    Altogether,
    \begin{equation*}
      \int_{-2}^2 (x+3) \sqrt{4-x^2}
      = \int_{-2}^2 \left( x\sqrt{4-x^2} + 3 \sqrt{4-x^2} \right) \;
      dx
      = \int_{-2}^2 x\sqrt{4-x^2} \; dx + 3 \int_{-2}^2 \sqrt{4-x^2}
      \; dx
      = 0 + 3(2\pi) = 6\pi
    \end{equation*}
  \item If we try the obvious substitution $u=1-x^4$, we are going to
    have difficulty completing it.  So instead, inspired by the
    previous problem, let's try $u=x^2$, $du/dx = 2x$, $du/2 = x \;
    dx$; when $x=0$, $u=x^2=0$, and when $x=1$, $u=x^2=1$:
    \begin{equation*}
      \int_0^1 x \; \sqrt{1-x^4} \; dx
      = \frac{1}{2} \int_{0}^{1} \sqrt{1-u^2} \; du
    \end{equation*}
    Geometrically, the integral is the area of one quarter of a unit
    circle, which is $\pi/4$, so the answer is
    \begin{equation*}
      \int_0^1 x \; \sqrt{1-x^4} \; dx
      = \frac{1}{2} \int_{0}^{1} \sqrt{1-u^2} \; du
      = \frac{1}{2} \cdot \frac{\pi}{4}
      = \frac{\pi}{8}
    \end{equation*}
  \end{enumerate}
\item
  \begin{enumerate}
  \item This one requires a trick.  Recall the Pythagorean identity
    $\cos^2 x = 1-\sin^2 x$.  We can write
    \begin{equation*}
      \int \cos^3 x \; \sin^6 x \; dx
      = \int \cos x \; (1-\sin^2 x) \; \sin^6 x \; dx
      = \int \cos x \; \sin^6 x \; dx  - \int \cos x \; \sin^8 x \; dx
    \end{equation*}
    Both of the resulting integrals can be evaluated by the
    substitution $u=\sin x$, $du = \cos x \; dx$:
    \begin{equation*}
      \int \cos x \; \sin^6 x \; dx - \int\cos x \; \sin^8 x \; dx
      = \int u^6 \; du - \int u^8 \; du
      = \frac{1}{7} \sin^7 x - \frac{1}{9} \sin^9 x + C
    \end{equation*}
    A similar strategy works for the integral of any product of a
    power of cosine times a power of sine, as long as at least one of
    the powers is odd.  If both powers are even, you need to use more
    advanced techniques you will learn in MATH 111.
  \item Let $u=-x$, $-du=dx$; note that when $x=-1$, $u=1$ and when
    $x=1$, $u=-1$.  Then
    \begin{equation*}
      \int_{-1}^1 \frac{x^2\; \tan x}{x^4+1} \; dx
      = \int_{1}^{-1} \frac{(-u)^2 \; \tan (-u)}{(-u)^4+1} (-du)
      = \int_{-1}^1 \frac{u\;(- \tan u)}{u^4+1} \; du
      = -\int_{-1}^1 \frac{ x\; \tan x}{x^4+1} \; dx
    \end{equation*}
    where we have used the fact that $\tan x$ is odd (i.e.,
    $\tan(-x) = -\tan x$), $x^2$ is even (i.e., $(-x)^2 = x^2$), $x^4$
    is even, and we used the property
    \begin{equation*}
      \int_a^b f(x) \; dx = -\int_b^a f(x) \; dx
    \end{equation*}
    of the Riemann integral.  In summary,
    \begin{equation*}
      \int_{-1}^1 \frac{x^2 \; \tan x}{x^4+1} \; dx
      = -\int_{-1}^1 \frac{x^2\; \tan x}{x^4+1} \; dx
    \end{equation*}
    which implies that the value of the integral is $0$.

    You can also reason about this problem geometrically; the
    integrand is odd, and the domain of integration is balanced across
    $0$, so the negative areas exactly balance the positive areas and
    the integral must be $0$. % EJD: Graph
  \end{enumerate}
\item Let $u=x^2$, $du/dx = 2x$, $du/2 = x\; dx$; note that when
  $x=0$, $u=x^2=0$, and when $x=3$, $u=x^2=9$.  So
  \begin{equation*}
    \int_0^3 xf(x^2)\; dx
    = \frac{1}{2} \int_0^9 f(u) \; du
    = \frac{1}{2} \cdot 4 = 2
  \end{equation*}
\item Let $u=\pi-x$, $du/dx = -1$, $-du = dx$, $x=\pi-u$; note that
  when $x=0$, $u=\pi-x=\pi$, and when $x=\pi$, $u=\pi-\pi=0$:
  \begin{equation*}
    \int_0^\pi x f(\sin x) \; dx
    = -\int_\pi^0 (\pi-u) f(\sin(\pi-u)) \; du
    = \int_0^\pi (\pi-u) f(\sin(\pi-u)) \; du
  \end{equation*}
  By the angle subtraction identity for $\sin$ we have
  \begin{equation*}
    \sin(\pi-u) = \sin\pi\cos u - \sin u \cos \pi
    = 0\cos u - \sin u (-1)
    = \sin u
  \end{equation*}
  so
  \begin{equation*}
    \int_0^\pi x f(\sin x) \; dx
    = \int_0^\pi (\pi-u) f(\sin(\pi-u)) \; du
    = \pi \int_0^\pi f(\sin u) \; du - \int_0^\pi u f(\sin u) \; du
  \end{equation*}
  Since $u$ is a dummy variable in the integral we can replace it by
  $x$:
  \begin{equation*}
    \int_0^\pi x f(\sin x) \; dx
    = \pi \int_0^\pi f(\sin x) \; dx - \int_0^\pi x f(\sin x) \; dx
  \end{equation*}
  We can move the last term to the left side of the equation to obtain
  \begin{equation*}
    2\int_0^\pi x f(\sin x) \; dx
    = \pi \int_0^\pi f(\sin x) \; dx
  \end{equation*}
  Dividing both sides of the equation above by $2$ gives the result.
\end{enumerate}
\end{document}