\documentclass{article}
\usepackage{amsmath}
\usepackage{fullpage}
\usepackage{graphicx}
\usepackage[aux]{rerunfilecheck}

\input{../common.tex}

\newcommand{\ds}{\displaystyle}

\title{\commonPSTitleZeroOneSix\ Solutions}
\author{\commonAuthor}
\date{\commonPSTitleZeroOneSix}

\begin{document}
\maketitle
\begin{enumerate}
\item %1
  \begin{enumerate}
  \item %a
    The following is an example of a completely rigorous argument for
    evaluating limits.  For an example of an argument which is not completely
    rigorous but would be acceptable, see the solution for part (b).
    
    By the quotient rule,
    \begin{equation*}
      \lim_{x\to 2} \frac{2x^2+1}{x^2+6x-4}
      = \frac{\lim_{x\to 2} (2x^2+1)}{\lim_{x\to 2}(x^2+6x-4)}
    \end{equation*}
    \emph{provided} both limits exist \emph{and provided} the limit
    in the quotient is not equal to zero.  Since we don't (officially)
    know whether those conditions hold, the equality in the above line
    is provisional for the time being.  We won't know whether those conditions
    hold until we reach the end of the calculation.

    % EJD: two many 2s
    To evaluate the numerator in the above calculation, we use the sum rule
    \begin{equation*}
      \lim_{x\to 2} (2x^2+1) = \lim_{x\to 2} 2x^2 + \lim_{x\to 2} 1
    \end{equation*}
    Again, we don't know whether the equality above holds until we finish
    calculating the limit.  We now use the constant multiple rule:
    \begin{equation*}
      \lim_{x\to 2} 2x^2 = 2\lim_{x\to 2} x^2
    \end{equation*}
    and the power rule
    \begin{equation*}
      \lim_{x\to 2} x^2 = (\lim_{x\to 2} x)^2
    \end{equation*}
    and finally the limit of $x$
    \begin{equation*}
      \lim_{x\to 2} x = 2
    \end{equation*}
    to obtain
    \begin{equation*}
      \lim_{x\to 2} (2x^2+1) = \lim_{x\to 2} 2x^2 + \lim_{x\to 2} 1
      = 2\left(\lim_{x\to 2} x\right)^2 + \lim_{x\to 2} 1
      = 2(2)^2 + 1 = 9
    \end{equation*}
    
    Similarly, to evaluate the denominator, we use the sum rule, the 
    constant multiple rule, the power rule, and the ``bottom level rules'' 
    for $\ds \lim_{x\to 2} x$ and $\lim_{x\to 2} c$ to obtain
    \begin{equation*}
      \lim_{x\to 2} (x^2+6x-4) = \lim_{x\to 2} x^2 + \lim_{x\to 2} 6x
      - \lim_{x\to 2} 4
      = \left(\lim_{x\to 2} x\right)^2 + 6 \lim_{x\to 2} x - \lim_{x\to 2} 4
      = 2^2 + 6(2) - 4 = 12
    \end{equation*}
    Note that the above limit is not $0$, so we can apply the quotient rule
    \begin{equation*}
      \lim_{x\to 2} \frac{2x^2+1}{x^2+6x-4}
      = \frac{\lim_{x\to 2} (2x^2+1)}{\lim_{x\to 2}(x^2+6x-4)}
      = \frac{9}{12} = \frac{3}{4}
    \end{equation*}
  \item %b
    % EJD: check numbers: different from text?
    We can express the same type of argument as in part (a)
    in a single line (provided we understand that every step
     is provisional until the whole argument is complete):
    \begin{align*}
      \lim_{t\to -1} (t^2+1)^3(t+3)^5
      &= \lim_{t\to -1} (t^2+1)^3 \times \lim_{t\to -1} (t+3)^5
      \\
      &= (\lim_{t\to -1} t^2+1)^3 \times (\lim_{t\to -1} (t+3))^5
      \\
      &= (\lim_{t\to -1} t^2 + \lim_{t\to -1} 1)^3 
      \times (\lim_{t\to -1} t+3)^5
      \\
      &= ((\lim_{t\to -1} t)^2 + \lim_{t\to -1} 1)^3
      \times (\lim_{t\to -1} t + 3 )^5
      \\
      &= ((-1)^2+1)^3 \times (-1+3)^5 = (1+1)^3 \times (2)^5 = 8\times 32
      = 256
    \end{align*}
  \end{enumerate}
\item %2
  \begin{enumerate}
  \item %a EJD: make different from textbook
    First, we should substitute $x=-4$ into the denominator; if the result
    is non-zero, we can find the answer to the question just with a straight
    substitution.  If the result is zero, we will probably have to factor.
    We have
    \begin{equation*}
      \left. x^2+3x-4 \right|_{x=-4}
      = (-4)^2 + 3(-4) - 4 = 16-12-4 = 0
    \end{equation*}
    so we will have to factor.  Note that
    \begin{align*}
      x^2+5x+4 &= (x+4)(x+1) \\
      x^2+3x-4 &= (x+4)(x-1)
    \end{align*}
    so we have
    \begin{equation*}
      \lim_{x\to -4} \frac{x^2+5x+4}{x^2+3x-4}
      = \lim_{x\to -4} \frac{(x+4)(x+1)}{(x+4)(x-1)}
      = \lim_{x\to -4} \frac{x+1}{x-1} 
      = \frac{-4+1}{-4-1}
      = \frac{-3}{-5} = \frac{3}{5}
    \end{equation*}
  \item %b EJD: make different from textbook
    As above, we check the value of the function
    when $x=1$: 
    \begin{equation*}
      \left. \frac{x^3-1}{x^2-1} \right|_{x=1}
      = \frac{1^3-1}{1^2-1} = \frac{0}{0}
    \end{equation*}
    so we have to do more work.  In this case we have to factor.
    The problem factor is $x-1$, so we try to pull a factor of that type 
    from both the numerator and the denominator.  In the numerator, we have
    \begin{equation*}
      x^3-1=(x-1)(x^2+x+1)
    \end{equation*}
    which you can memorize as a common, useful factorization, or you can obtain
    by polynomial division.  In the denominator we have
    \begin{equation*}
      x^2-1 = (x-1)(x+1)
    \end{equation*}
    by the standard difference of squares factorization.  Evaluating the limit
    we have
    \begin{equation*}
      \lim_{x\to 1} \frac{x^3-1}{x^2-1} 
      = \lim_{x\to 1} \frac{(x-1)(x^2+x+1)}{(x-1)(x+1)}
      = \lim_{x\to 1} \frac{x^2+x+1}{x+1}
      = \frac{1^2+1+1}{1+1} = \frac{3}{2}
    \end{equation*}
  \item %c EJD: make different from text
    Again, we first check what happens when we substitute $h=0$ into the
    expression.  We have
    \begin{equation*}
      \left. \frac{\sqrt{1+h}-1}{h} \right|_{h=0}
      = \frac{\sqrt{1+0}-1}{0} = \frac{0}{0}
    \end{equation*}
    so we have to do more work.
    To evaluate limits involving square roots, we often find it helpful to 
    multiply by the ``conjugate radical'', in this case $\sqrt{1+h} + 1$:
    \begin{multline*}
      \lim_{h\to 0} \frac{\sqrt{1+h}-1}{h}
      = \lim_{h\to 0} \frac{\sqrt{1+h}-1}{h} \cdot 
      \frac{\sqrt{1+h}+1}{\sqrt{1+h}+1}
      = \lim_{h\to 0} \frac{1+h - 1}{h(\sqrt{1+h}+1)}
      \\
      = \lim_{h\to 0} \frac{h}{h(\sqrt{1+h}+1)}
      = \lim_{h\to 0} \frac{1}{\sqrt{1+h}+1} 
      = \frac{1}{\sqrt{1+0}+1} = \frac{1}{2}
    \end{multline*}
  \item %d
    Again, substituting $h=0$ gives an expression of the form $0/0$, so we
    have to do more work.  We rewrite the negative power as a fraction, and
    then clear fractions:
    \begin{multline*}
      \lim_{h\to 0} \frac{(3+h)^{-1} - 3^{-1}}{h}
      = \lim_{h\to 0}\frac{\frac{1}{3+h}-\frac{1}{3}}{h}
      = \lim_{h\to 0} \left(\frac{3}{3(3+h)}-\frac{3+h}{3(3+h)}\right) 
      \frac{1}{h}
      \\
      = \lim_{h\to 0} \left(\frac{3-(3+h)}{3(3+h)}\right) \frac{1}{h}
      = \lim_{h\to 0} \frac{-h}{3(3+h)} \frac{1}{h}
      = \lim_{h\to 0} \frac{-1}{3(3+h)}
      = -\frac{1}{3(3+0)} = -\frac{1}{9}
    \end{multline*}
  \end{enumerate}
%% \item %3 FIXME : from 2.5
%%   \begin{enumerate}
%%   \item %a
%%     Each of the multiplicands $\sqrt[3]{x}$ and $1+x^2$ is defined and 
%%     continuous for all real numbers $x$, the former because it is a root
%%     function with an odd index $3$, the latter because it is a polynomial,
%%     so the product function $G$ is also defined and continuous for all real
%%     numbers.
%%   \item %b
%%     The sine function is defined and continuous for all real numbers (that
%%     is just a fact you should memorize), and the function $x+1$ is defined
%%     for all real numbers, but we have to be careful about when the denominator
%%     $x+1$ is $0$.  Solving the equation $x+1=0$ we get $x=-1$ as a value for
%%     which the quotient $\sin x/(x+1)$ is undefined, and hence not continuous.
%%     However, $x=-1$ is outside of the domain of the function, so we can still
%%     say that the function is continuous for all values of $x$ on the domain.
%%   \item %c
%%     We can break the given function down as the composition of the tangent
%%     function $\tan u$ and the ``doubling'' function $d(x)=2x$: 
%%     \begin{equation*}
%%       h(x) = \tan (2x) = \tan (d(x)) \implies h = \tan \circ d
%%     \end{equation*}
%%     The $\tan$ function is continuous wherever it is defined, and the doubling
%%     function is a polynomial so it is continuous everywhere.  Finally,
%%     the composition of two continuous functions is continuous where it is
%%     defined, namely wherever $2x\ne (2k+1)\pi/2$ or $x\ne (2k+1)\pi/4$.
%%   \item %d
%%     The sine and cosine functions are defined and continuous everywhere, so
%%     the composition 
%%     \begin{equation*}
%%       \sin\circ \cos \circ \sin
%%     \end{equation*}
%%     is also defined and continuous everywhere.
%%   \end{enumerate}
%% \item %4 FIXME : from 2.5
%%   \begin{enumerate}
%%   \item %a
%%     When $x\ne 3$, the function $f(x)$ is the same as 
%%     \begin{equation*}
%%       \frac{2x^2-5x-3}{x-3}
%%     \end{equation*}
%%     which is continuous for $x\ne 3$, so it follows that $f(x)$ is continuous
%%     for $x\ne 3$.  So the only number in question is $x=3$.  Calculating the
%%     limit by factoring,
%%     \begin{equation*}
%%       \lim_{x\to 3} f(x) = \lim_{x\to 3} \frac{2x^2-5x-3}{x-3}
%%       = \lim_{x\to 3} \frac{(x-3)(2x+1)}{x-3}
%%       = \lim_{x\to 3} (2x+1) = 7
%%     \end{equation*}
%%     while on the other hand $f(3)=6$.  Since $\ds \lim_{x\to 3} f(x)\ne f(3)$,
%%     $f$ is not continuous at $x=3$.  (You should be able to graph $f$ easily.
%%     How could you change the definition of $f$ to make it continuous?)
%%   \item %b
%%     The function $x+1$ is continuous everywhere, so it is continuous on the
%%     interval $-\infty< x< 1$.  Similarly, $1/x$ is continuous everywhere
%%     except $x=0$, so it is continuous on the interval $1<x<3$.  Finally,
%%     $\sqrt{x-3}$ is continuous wherever it is defined, so it is continuous
%%     on the interval $3< x<\infty$.  So the only places where $g$ might
%%     not be continuous are $x=1$ and $x=3$.  At $x=1$ we have
%%     \begin{align*}
%%       \lim_{x\to 1^-} g(x) &= \lim_{x\to 1^-} (x+1) = 2 \\
%%       g(1) &= \left. x+1 \right|_{x=1} = 1+1 = 2 \\
%%       \lim_{x\to 1^+} g(x) &= \lim_{x\to 1^+} \frac{1}{x} = \frac{1}{1} = 1
%%     \end{align*}
%%     Since not all of the above results agree, the function $g(x)$ is not
%%     continuous at $x=1$.  At $x=3$ we have
%%     \begin{align*}
%%       \lim_{x\to 3^-} g(x) &= \lim_{x\to 3^-} \frac{1}{x} = \frac{1}{3} \\
%%       g(3) &= \sqrt{3-3} = \sqrt{0} = 0 \\
%%       \lim_{x\to 3^+} g(x) &= \lim_{x\to 3^+} \sqrt{x-3} = \sqrt{3-3} = 0
%%     \end{align*}
%%     Again, not all of the above results agree, so the function $g(x)$ is not
%%     continuous at $x=3$.
%%   \end{enumerate}
%% \item %5 FIXME : from 2.5
%%   \begin{enumerate}
%%   \item %a
%%     We convert the problem to one of showing the existence of a zero
%%     of the function by rewriting the equation as $\sqrt[3]{x} +x - 1 = 0$.
%%     Then we have to show that the function $f(x)=\sqrt[3]{x}+x-1$ has a 
%%     zero on the interval $(0,1)$.  

%%     The Intermediate Value Theorem does not apply directly to the above
%%     situation because the interval $(0,1)$ is not a closed interval, but
%%     an open interval.  However, in this case we can 
%%     widen the interval slightly to $[0,1]$ because we can't add any roots
%%     of the function because 
%%     \begin{align*}
%%       f(0) &= \sqrt[3]{0} + 0 - 1 = 0 + 0 - 1 = -1 \ne 0 \\
%%       f(1) &= \sqrt[3]{1} + 1 - 1 = 1 + 1 - 1 = 1 \ne 0
%%     \end{align*}
%%     So if $f$ has a root on $[0,1]$ it must have a root on $(0,1)$.

%%     Note that $f$ is continuous (why?) and $f(0)<0$, $f(1)>1$, so by the 
%%     IVT $f$ has a root in the interval $(0,1)$.
%%   \item %b
%%     This was done in the lecture.
%%   \item %c
%%     We must show that the function $f(x)=x^5-x^2+2x+3$ has a root on the
%%     interval $(-\infty,\infty)$.  In this case we can't widen the interval
%%     by including $-\infty$ and $\infty$ because those are not numbers.
%%     So we must consider a smaller closed interval inside $(-\infty,\infty)$.
%%     We just try to guess appropriate bounds for the interval, and if they
%%     don't work, we guess again.  Note that $f(0)=0^5-0^2+2(0)+3>0$ so if
%%     we can find a value $a$ at which $f(a)<0$ then we can apply the IVT.
%%     Try $f(-1)=(-1)^5-(-1)^2+2(-1)+3=-1-1-2+3=-1<0$ so we're in luck.  The
%%     function $f(x)$ changes sign on the closed interval $[-1,0]$, and it
%%     is continuous because it's a polynomial, so the IVT applies and $f(x)$
%%     has a root in the interval $(-1,0)$ so it has a root in the bigger
%%     interval $(-\infty,\infty)$.
%%   \end{enumerate}
%% \item %6 FIXME : from 2.5
%%   As in a previous question, $f(x)$ is continuous in the open intervals
%%   $(-\infty,2)$, $(2,3)$, and $(3,\infty)$ because the functions 
%%   $(x^2-4)/(x-2)$, $ax^2-bx+3$, and $2x-a+b$ are continuous on those
%%   intervals, respectively.  So we just have to pay attention to what happens
%%   near $x=2$ and $x=3$.  Near $x=2$ we have
%%   \begin{align*}
%%     \lim_{x\to 2^-} f(x) &= \lim_{x\to 2^-} \frac{x^2-4}{x-2}
%%     = \lim_{x\to 2^-} \frac{(x-2)(x+2)}{x-2} = \lim_{x\to 2^-} (x+2) = 4 \\
%%     f(2) &= a(2)^2-b(2)+3 = 4a-2b+3 \\
%%     \lim_{x\to 2^+} f(x) &= \lim_{x\to 2^+} (ax^2-bx+3) = a(2)^2-b(2)+3
%%     = 4a-2b+3
%%   \end{align*}
%%   so the condition for $f$ to be continuous at $x=2$ is $4a-2b+3=4$ or
%%   $4a-2b=1$.  Similarly, near $x=3$ we have
%%   \begin{align*}
%%     \lim_{x\to 3^-} f(x) &= \lim_{x\to 3^-} (ax^2-bx+3) = a(3)^2-b(3)+3 = 
%%     9 a -3 b + 3 \\
%%     f(3) &= 2(3)-a+b = 6-a+b \\
%%     \lim_{x\to 3^+} f(x) &= \lim_{x\to 3^+} (2x-a+b) = 2(3)-a+b = 6-a+b
%%   \end{align*}
%%   so the condition for $f$ to be continuous at $x=3$ is $9a-3b+3=6-a+b$ or
%%   $10a-4b=3$.  In summary our conditions are
%%   \begin{align*}
%%     4a-2b&=1 \\
%%     10a-4b&=3
%%   \end{align*}
%%   which is a linear system in the two variables $a$ and $b$.  Multiplying the
%%   first equation by $-2$ and adding, $2a=1$ so $a=1/2$, which implies $b=1/2$.
% EJD: add more questions?
\item %3 EJD: check numbers vs. textbook
  This question calls for the squeeze theorem.  We need to separate the 
  function into two parts, one of which is bounded and the other of which
  tends to $0$ (``vanishes'')
  as $x\to 0^+$.  We have $\sin^2(2\pi/x)\ge 0$ because squares
  are always nonnegative, and $\sin^2(2\pi x)\le 1$ because the sine of 
  anything is between $-1$ and $1$, so we can write
  \begin{equation*}
    0\le \sin^2(2\pi/x) \le 1 \implies 1 \le 1+\sin^2(2\pi/x) \le 2
  \end{equation*}
  which gives our bounded part.  On the other hand, $\sqrt{x}\to 0$ as
  $x\to 0^+$ which gives our ``vanishing'' part, and multiplying the 
  above inequality by $\sqrt{x}$ we can write
  \begin{equation*}
    1\sqrt{x} \le \sqrt{x}(1+\sin^2(2\pi/x)) \le 2\sqrt{x}
  \end{equation*}
  Note that $\sqrt{x}\ge 0$ for $x>0$ so the above inequality does not 
  ever reverse.  Now since $\sqrt{x}\to 0$ as $x\to 0^+$, and similarly
  $2\sqrt{x}\to 0$ as $x\to 0^+$, the squeeze theorem tells us that the
  part squeezed in the middle of the above inequality 
  also $\to 0$ as $x\to 0^+$, so we conclude
  \begin{equation*}
    \lim_{x\to 0^+} \sqrt{x}(1+\sin^2(2\pi/x)) = 0
  \end{equation*}
\item %4 EJD: check numbers against textbook
  Just substituting $x=2$ into the function gives the expression $0/0$ so
  we must do some more work before we can get an answer.  In expressions
  involving radicals (square roots) we often find it helpful to multiply
  by the conjugate radical.  In this case there are two radicals so we 
  multiply by them both, one at a time.  We have
  \begin{equation*}
    \frac{\sqrt{6-x}-2}{\sqrt{3-x}-1}
    = \frac{\sqrt{6-x}-2}{\sqrt{3-x}-1} \cdot \frac{\sqrt{6-x}+2}{\sqrt{6-x}+2}
    = \frac{6-x-4}{(\sqrt{3-x}-1)(\sqrt{6-x}+2)}
    = \frac{2-x}{(\sqrt{3-x}-1)(\sqrt{6-x}+2)}
  \end{equation*}
  Repeating the procedure with the second conjugate radical,
  \begin{multline*}
    \frac{2-x}{(\sqrt{3-x}-1)(\sqrt{6-x}+2)}
    = \frac{2-x}{(\sqrt{3-x}-1)(\sqrt{6-x}+2)} \cdot 
    \frac{\sqrt{3-x}+1}{\sqrt{3-x}+1}
    \\
    = \frac{(2-x)(\sqrt{3-x}+1)}{(3-x-1)(\sqrt{6-x}+2)}
    = \frac{(2-x)(\sqrt{3-x}+1)}{(2-x)(\sqrt{6-x}+2)}
    = \frac{\sqrt{3-x}+1}{\sqrt{6-x}+2}
  \end{multline*}
  Taking the limit we have
  \begin{equation*}
    \lim_{x\to 2} \frac{\sqrt{6-x}-2}{\sqrt{3-x}-1}
    = \lim_{x\to 2} \frac{\sqrt{3-x}+1}{\sqrt{6-x}+2}
    = \frac{\sqrt{3-2}+1}{\sqrt{6-2}+2} = \frac{2}{4} = \frac{1}{2}
  \end{equation*}
\end{enumerate}
\end{document}

