%\documentclass{article}
%\usepackage{beamerarticle}
\documentclass[serif,ignorenonframetext]{beamer}

\input{../common.tex}

\usepackage{mathptmx}
\usepackage{multirow}
\usepackage{tikz}

\newcommand{\ds}{\displaystyle}

\mode<article>{}
\mode<presentation>{\usetheme{\commonTheme}\usecolortheme{\commonColorTheme}}

\title{\commonTitleZeroTwoThree}
\subtitle{\commonSubtitleZeroTwoThree}
\author{\commonAuthor}
\institute{\commonInstitute}
\date{\commonDateZeroTwoThree}


\begin{document}

%\section*{Outline}

\begin{frame}
  \titlepage
\end{frame}

\begin{frame}
  \frametitle{Contents}
  \tableofcontents
\end{frame}

\section{Differentiation Formulas}

\begin{frame}
  \frametitle{Review of the Reduction Strategy for Limits}
  \begin{itemize}[<+->]
  \item Recall when we evaluated limits, we applied limit laws
    to break a complicated limit into simpler parts.
  \item For example, we can apply the sum rule to the limit
    \begin{displaymath}
      \lim_{x\to 2} (3x+7) = \lim_{x\to 2} (3x) + \lim_{x\to 2} 7
    \end{displaymath}
    to break a complicated limit into simpler parts.
  \item Thee first summand can be broken down further by the 
    product rule for limits:
    \begin{displaymath}
      \lim_{x\to 2} (3x) 
      = (\lim_{x\to 2} 3) (\lim_{x\to 2} x )
    \end{displaymath}
  \item The resulting simple limits
    can be evaluated by applying the bottom level rules $\ds\lim_{x\to 2} c
    = c$ for $c=3$ and $c=7$, and $\ds \lim_{x\to 2} x = 2$.
  \item We would like to develop a similar strategy for evaluating derivatives.
  \end{itemize} 
\end{frame}


\subsection{Bottom Level Rules for Derivatives}

\begin{frame}
  \frametitle{Bottom Level Rules for Derivatives: Constant Functions}
  \begin{itemize}[<+->]
  \item Let us begin this time with some bottom-level rules for derivatives.
  \item These rules are slightly different from the corresponding rules for
    limits.
  \item First, suppose $f(x)=c$, a constant.  Then
    \begin{align*}
      \frac{d}{dx} f(x) 
      \uncover<+->{= \lim_{h\to 0} \frac{f(x+h) - f(x)}{h}  }
      \uncover<+->{= \lim_{h\to 0} \frac{c - c}{h} }
      \uncover<+->{= \lim_{h\to 0} \frac{0}{h} }
      \uncover<+->{= 0}
    \end{align*}
  \item In words, the derivative of a constant is $0$.
  \end{itemize}
\end{frame}

\begin{frame}
  \frametitle{Bottom Level Rules for Derivatives: the Identity Function}
  \begin{itemize}[<+->]
  \item Now let $f(x)=x$.  That function is known as the `identity
    function' because the output of $f$ is identical to the input.
  \item Now, calculating the derivative,
    \begin{align*}
      f'(x) 
      \uncover<+->{= \lim_{h\to 0} \frac{f(x+h) - f(x)}{h}  }
      \uncover<+->{= \lim_{h\to 0} \frac{x+h - x}{h} }
      \uncover<+->{= \lim_{h\to 0} \frac{h}{h} }
      \uncover<+->{= 1}
    \end{align*}
  \item In words, the derivative of the identity function is $1$.
  \item The derivatives of constant functions and of the identity
    function will be the building blocks for most of the derivative
    calculations in this section.
  \item There are other bottom-level derivatives that we will learn later.
    Each time we introduce a new kind of function (e.g., 
    $\sin$, $\cos$, $\exp$, $\log$, \ldots) there
    will be a new bottom-level derivative that will have to be calculated
    from first principles.  
  \end{itemize}
\end{frame}


\subsection{Reduction Formulas for Derivatives}

\begin{frame}
  \frametitle{Sums, Differences, and Constant Multiples for Derivatives}
  \begin{itemize}[<+->]
  \item As with limits, derivatives behave in a simple way with respect
    to sums, differences, and constant multiples.
  \item The derivative of a sum is the sum of the derivatives
    \begin{displaymath}
      (f+g)' = f'+g' \quad\mbox{or}\quad 
      \frac{d}{dx} (f(x)+g(x)) = \frac{d}{dx} f(x) + \frac{d}{dx} g(x)
    \end{displaymath}
  \item The derivative of a difference is the difference of the derivatives.
    \begin{displaymath}
      (f-g)' = f' - g' \quad\mbox{or}\quad
      \frac{d}{dx} (f(x)-g(x)) = \frac{d}{dx} f(x) - \frac{d}{dx} g(x)
    \end{displaymath}
  \item The derivative of a constant multiple is the constant multiple of
    the derivative.
    \begin{displaymath}
      (cf)' = cf' \quad\mbox{or}\quad
      \frac{d}{dx} (cf(x)) = c\frac{d}{dx} f(x)
    \end{displaymath} 
  \end{itemize}
\end{frame}

\begin{frame}
  \frametitle{Justifying the Sum Rule for Derivatives}
  \begin{itemize}[<+->]
  \item The sum, difference, and constant multiple rules are direct
    consequences of the corresponding rules for limits.
  \item For example, we have
    \begin{align*}
      (f+g)'(x)
      \uncover<+->{&= \lim_{h\to 0} \frac{(f+g)(x+h) - (f+g)(x)}{h} \\ }
      \uncover<+->{&= \lim_{h\to 0} \frac{f(x+h) + g(x+h) - f(x) - g(x)}{h} \\}
      \uncover<+->{&= \lim_{h\to 0} \left(\frac{f(x+h) - f(x)}{h}
        + \frac{g(x+h)-g(x)}{h} \right)}
    \end{align*}
  \item Now we apply the sum rule for limits to show the latter expression
    is the same as $f'(x)+g'(x)$.
  \end{itemize}
\end{frame}

\begin{frame}
  \frametitle{First Attempt at a Product Rule for Derivatives}
  \begin{itemize}[<+->]
  \item We've had some success we've had in guessing rules for derivatives
    from rules from the rules for limits.
  \item It might seem natural to guess that the derivative of a product is
    the product of the derivatives.
  \item That is incorrect, however.  Consider the example $f(x)=1$, $g(x)=x$.
  \item The derivative of the product is the derivative of $x$ which is $1$.
  \item The derivative of $f(x)$ is $0$ and the derivative of $g(x)$ is $1$,
    so the product of the derivatives is $0$.
  \item Even in this simple case, the derivative of the product ($1$) is
    different from the product of the derivatives ($0$).
  \item What is the correct rule?
  \end{itemize}
\end{frame}

\begin{frame}
  \frametitle{Discovering the Product Rule for Derivatives}
  \begin{itemize}[<+->]
  \item The product rule for derivatives is not what we might
    naively expect. 
    $(fg)'$ \textbf{is not} $f'g'$!
  \item To understand what the derivative of a product should be,
    consider the meaning of the derivative.  If I change $x$ by
    a small amount $dx$, this is what happens to $f$:
    \begin{displaymath}
      f(x+dx) = f(x) + f'(x) dx + \mbox{terms in $dx^2$, etc.}
    \end{displaymath}
  \item Now consider what happens to the product $f(x)g(x)$
    when we change $x$ by a small amount $dx$:
    \begin{align*}
      f(x+dx)g(x+dx) &= (f(x)+f'(x)dx+\cdots)(g(x)+g'(x)dx+\cdots) \\
      &= f(x)g(x) + 
      \tikz[baseline=(t1.base)]{
        \node[fill=yellow!50] (t1)
	{$(f'(x)g(x)+f(x)g'(x))$};
      }
      dx + \cdots
    \end{align*}
  \item This tells us that $(f(x)g(x))'$ should be $f'(x)g(x)+f(x)g'(x)$.
  \end{itemize}
\end{frame}

\begin{frame}
  \frametitle{The Product Rule for Derivatives}
  \begin{itemize}[<+->]
  \item In summary, we have the formula in Leibniz notation
    \begin{displaymath}
      \frac{d}{dx} \left(f(x)g(x)\right) 
      = \left(\frac{d}{dx} f(x)\right) g(x) 
      + f(x) \left(\frac{d}{dx} g(x) \right)
    \end{displaymath}
  \item Or, in more compact Newton notation,
    \begin{displaymath}
      (fg)' = f'g + fg'
    \end{displaymath}
  \item Note that the derivative of a product \textbf{is not} the product
    of the derivatives!
  \item Derivatives differ from limits in this regard.
  \end{itemize}
\end{frame}

\begin{frame}
  \frametitle{Discovering the Quotient Rule for Derivatives}
  \begin{itemize}[<+->]
  \item In a similar way, the quotient rule for derivatives is not what
    we might naively expect.  Consider $f(x)=x$, $g(x)=x$.  Then 
    $(f/g)'=0$ but $f'/g'=1$.
  \item We can figure out what the correct rule must be by differentiating
    the equation $f=g(f/g)$ using the product rule.
  \item We have $f'=g'(f/g) + g(f/g)'$.
  \item Solving for $(f/g)'$, we have
    \begin{align*}
      \left(\frac{f}{g}\right)'
      = \frac{gf'-fg'}{g^2}
    \end{align*}
  \item The mantra ``bottom times derivative of top minus top times derivative
    of bottom over bottom squared'' may help you remember the quotient rule.
  \end{itemize}
\end{frame}

%\begin{frame}
%  \frametitle{The Quotient Rule for Derivatives}
%  EJD
%\end{frame}

\begin{frame}
  \frametitle{Example: Derivatives of Monomials}
  \begin{itemize}[<+->]
  \item We now know enough to do some complicated 
    derivatives.
  \item Consider the derivative of $x^2$.  We can write
    $x^2$ as a product $x\cdot x$.
  \item The product rule then tells us that
    \begin{displaymath}
      \frac{d}{dx} x^2 = \frac{d}{dx} (x\cdot x)
      = \left( \frac{d}{dx} x \right) x + x \left(\frac{d}{dx} x\right)
      = x + x = 2x
    \end{displaymath}
  \item Using the previous result, the product rule tells us that
    \begin{displaymath}
      \frac{d}{dx} x^3 = \frac{d}{dx} (x\cdot x^2)
      = \left(\frac{d}{dx} x \right) x^2 + x\left(\frac{d}{dx} x^2\right)
      = x^2 + x\cdot 2x = 3x^2
    \end{displaymath}
  \item Continuing the pattern, we have $\ds \frac{d}{dx} x^n = nx^{n-1}$
    for $n=1,2,\ldots$.
  \item That result is found in a more complicated way in the textbook.
  \end{itemize}
\end{frame}

\begin{frame}
  \frametitle{Example: Power Rule for Derivatives}
  \begin{itemize}[<+->]
  \item We can now find derivatives of negative powers of $x$ using
    the quotient rule.
  \item Suppose $f(x) = x^{-m}$ where $m$ is some positive integer.
  \item We can write $f(x)=1/x^m$.  Differentiating by the quotient rule
    we have 
    \begin{displaymath}
      f'(x) = \frac{x^m (1)' - 1 (x^m)'}{(x^{m})^2}
      = \frac{-mx^{m-1}}{x^{2m}}
      = -m\frac{1}{x^{m+1}}
      = -mx^{-m-1}
    \end{displaymath}
  \item Writing $n=-m$ we have $\ds \frac{d}{dx} x^n = nx^{n-1}$ for 
    $n=-1,-2,\ldots$.
  \item The case $n=0$ is special, but the result still holds.
  \item In general, $\ds\frac{d}{dx} x^p = px^{p-1}$ for any real number
    $p$, but the proof is too complicated to give now.
  \end{itemize}
\end{frame}


\subsection{Application: Tangent and Normal Lines}

\begin{frame}
  \frametitle{Tangent Lines Revisited}
  \begin{columns}
  \column{0.65\textwidth}
  \begin{itemize}[<+->] 
  \item Now we can more easily solve derivative questions.
  \item Consider $f(x)=x^2+1$.  What is the tangent line at $a=1$?
  \item Recall that the tangent line is $y-f(a)=f'(a)(x-a)$.
  \item We know $f(a)$.  From our rules, 
    $\ds  \frac{d}{dx} f(x) 
    = \frac{d}{dx} (x^2 + 1) 
    = \frac{d}{dx} x^2 + \frac{d}{dx} 1
    = 2x + 0 = 2x$.
  \item So $f'(a)=f'(1)=2(1)=2$, and the 
    tangent line is $y-2=2(x-1)$.
  \end{itemize}
  \column{0.35\textwidth}
  \only<1-4>{\includegraphics[width=\textwidth]{perp2.eps}}%
  \only<5->{\includegraphics[width=\textwidth]{perp3.eps}}%
  \end{columns}
\end{frame}

\begin{frame}
  \frametitle{Perpendicular Lines}
  \begin{columns}
  \column{0.65\textwidth}
  \begin{itemize}[<+->]
  \item We will need to find lines which are \textbf{perpendicular}
    to a tangent line.
  \item Two lines are perpendicular if the product of their slopes is $-1$.
  \item E.g., if we have two lines $y=m_1x+b$
    and $y-y_0=m_2(x-x_0)$, they are perpendicular if $m_1m_2=-1$.
  \item Given the slope $m_1$ of a line, the slope $m_2$ of any perpendicular
    line is the \textbf{negative reciprocal} 
    of $m_1$: $\ds m_2 = -\frac{1}{m_1}$
  \end{itemize}
  \column{0.35\textwidth}
  \only<1>{\includegraphics[width=\textwidth]{perp0.eps}}%
  \only<2->{\includegraphics[width=\textwidth]{perp1.eps}}%
  \end{columns}
\end{frame}

\begin{frame}
  \frametitle{Normal Lines}
  \begin{columns}
  \column{0.65\textwidth}
  \begin{itemize}[<+->]
  \item Now we can find \textbf{normal lines} (lines perpendicular
    to a tangent at a point on a curve).  Let $f(x)=x^2+1$ and $a=1$.
  \item The slope of the tangent is $f'(1)=2(1)=2$;
    the slope of the normal line is $m_2=-1/2$.
  \item The normal line in point-slope form is
    $\ds  y-f(a)=m_2(x-a) $, or filling in the blanks,
    \uncover<+->{$y-2 = -\frac{1}{2}(x-1)$.}
  \item The normal line to $y=f(x)$ at $P(a,f(a))$ is 
    $\ds  y-f(a) = -\frac{1}{f'(a)} (x-a)$.
  \end{itemize}
  \column{0.35\textwidth}
  \only<1>{\includegraphics[width=\textwidth]{perp2.eps}}%
  \only<2>{\includegraphics[width=\textwidth]{perp3.eps}}%
  \only<3->{\includegraphics[width=\textwidth]{perp4.eps}}%
  \end{columns}
\end{frame}


\subsection{Examples and Exercises}

\begin{frame}
  \frametitle{Examples}
  \begin{enumerate}
  \item Calculate $y'$ where 
    \begin{enumerate}
    \item $\ds y=\sqrt{x} + \frac{1}{\sqrt[3]{x^4}}$
    \item $\ds y=\frac{3x-2}{\sqrt{x}}$.
    \item $\ds y=\frac{\sqrt{x}}{3x-2}$.
    \end{enumerate}
  \item Find the equations of the tangent and normal lines to the
    curve $\ds y=\frac{x-1}{x+1}$ at the point $(0,-1)$.
  \item Find the equations of the tangent and normal lines to the 
    curve $\ds y=\frac{x^2-1}{x^2+1}$ at the point $(0,-1)$.
  \end{enumerate}
\end{frame}

\begin{frame}
  \frametitle{Solution to Example 3}
  \begin{itemize}
  \item In this example we have 
    $\ds y'=\frac{(x^2+1)2x - (x^2-1)2x}{(x^2+1)^2}
    = \frac{4x}{(x^2+1)^2}$, so $y'(0)=0$.  
  \item The equation of the tangent
    line is easy enough to find: $y-f(a)=f'(a)(x-a)$ where $a=0$, $f(a)=-1$,
    and $f'(a)=0$ gives $y-(-1)=0(x-0)$ or in other words $y=-1$.
  \item The equation of the normal is not so clear in this case.  Since 
    the slope of the tangent is $0$, the slope of the normal would be
    $-1/0$ which doesn't make any sense.  However, it should seem clear that
    a line perpendicular to the horizontal line $y=-1$ is a vertical line.
    Since the vertical line must pass through $(0,1)$, the
    equation of the normal line is $x=0$.  Draw it!
  \end{itemize}
\end{frame}

\begin{frame}
  \frametitle{Exercises}
  Now you should work on Problem Set~2.3.  After you have finished it,
  you should try the following additional exercises from Section~2.3:
  \begin{itemize}
  \item[2.3] 
    C-level: 1--22, 25--44, 51--52, 53--54, 55--58, 59--62, 63--66 \\
    B-level: 23--24, 45, 46--48, 49--50, 67, 68, 69--72, 73--74, 75--76,
    77--82, 83--86, 93--96, \\
    A-level: 87, 88--92, 97--100, 101--110
  \end{itemize}
 \end{frame}


\end{document}

