\documentclass{article}
\usepackage{amsmath}
\usepackage{fullpage}
%\usepackage{graphicx}
\usepackage{tikz}
\usepackage[aux]{rerunfilecheck}

\input{../common.tex}

\newcommand{\ds}{\displaystyle}

\title{\commonPSTitleZeroOneOne\ Solutions}
\author{\commonAuthor}
\date{\commonDateZeroOneOne}

\begin{document}
\maketitle
\begin{enumerate}
\item %1
  We have
  \begin{align*}
    f(2) &= 3(2)^2-2+2 = 3\cdot 4 = 12 \\
    f(-2) &= 3(-2)^2-(-2) + 2 = 3(4) + 2 + 2 = 12 + 4 = 16 \\
    f(a) &= 3a^2-a+2 \\
    f(-a) &= 3(-a)^2 -(-a) + 2 = 3a^2 + a + 2 \\
    f(a+1) &= 3(a+1)^2 - (a+1) + 2 = 3(a^2+2a+1) - a - 1 + 2
    = 3a^2 + 6a + 3 - a + 1 = 3a^2+5a+4 \\
    2f(a) &= 2(3a^2-a+2) = 6a^2-2a+4 \\
    f(2a) &= 3(2a)^2-(2a) + 2 = 3(4a^2) - 2a + 2 = 12a^2-2a+2 \\
    f(a^2) &= 3(a^2)^2 - (a^2) + 2 = 3a^4-a^2+ 2 \\
   (f(a))^2 &= (3a^2-a+2)^2 = 9a^4 -3a^3 + 6a^2 -3a^3+a^2-2a+6a^2-2a+4
    = 9a^4-6a^3+12a^2-4a+4 \\
    f(a+h) &= 3(a+h)^2 - (a+h) + 2 = 3(a^2 + 2ah + h^2) -a-h+2 = 
    3a^2+6ah+3h^2-a-h+2
  \end{align*}
  For this question, I will accept correct 
  answers that do not involve simplification, but you will need to be able
  to do those simplifications when we calculate derivatives in chapters 2
  and 3.
\item %2
  We can build up the calculation in steps.  We have $f(x)=1/x$, $f(a)=1/a$,
  so the numerator is
  \begin{equation*}
    f(x)-f(a) = \frac{1}{x} - \frac{1}{a} = \frac{a}{ax} - \frac{x}{ax}
    = \frac{a-x}{ax}
  \end{equation*}
  where I subtracted fractions by putting them over a common denominator.
  It follows that the difference quotient is
  \begin{equation*}
    \frac{f(x)-f(a)}{x-a} = \left(f(x)-f(a)\right) \cdot \frac{1}{x-a}
    = \frac{a-x}{ax} \cdot \frac{1}{x-a} = \frac{-1}{ax}
  \end{equation*}
\item \label{q:cases} %3 
  We first graph the line $y=x+2$ on the domain $x\le -1$ by finding two
  points on the line.  We select $x=-1$ which gives $y=x+2=-1+2=1$, so
  we plot the point $(x,y)=(-1,1)$.  Next we choose another $x$ value $\le -1$,
  say $x=-3$ which gives $y=x+2=-3+2=-1$, so we plot the point $(x,y)=(-3,-1)$.
  We draw a line segment connecting those two points, which graphs the
  function for $x\le -1$.

  Next, we graph the parabola $y=x^2$ on the domain $x>-1$.  That is a 
  standard parabola curve, and you should know that it opens upwards
  (or you can see that because the coefficient of $x^2$ is $+1$, a positive
  number); that it has vertex $(0,0)$; and that it passes through a 
  collection of points $(-1,1)$, $(0,0)$, $(1,1)$, $(2,4)$, and so on.
  Note that $(-1,1)$ isn't on the parabola, which has 
  domain $x>-1$, so technically we should draw an open circle at $(-1,1)$
  on the parabola; however, the point $(-1,1)$ is on the linear part of
  the curve.  Because the curves join together, we don't have to draw either
  the open dot that goes with the parabola nor the closed dot that goes
  with the linear curve.

  See Figure~\ref{fig:cases} for the final result.
  \begin{figure}[htbp]
    \centering
    \begin{tikzpicture}[yscale=0.5]
      \draw[very thin,color=gray] (-3.1,-1.1) grid (2.9,9.1);

      \draw[->,thick] (-3.2,0) -- (3.2,0) node[right] {$x$};
      \draw[->,thick] (0,-0.2) -- (0,9.2) node[above] {$y$};

      \draw[color=orange,domain=-3:-1] plot (\x,{\x+2});
      \draw[color=orange,domain=-1:3] plot (\x,{\x * \x}) node[left] {$y=f(x)$};
    \end{tikzpicture}
    \caption{Graph of $y=f(x)$ from question~\ref{q:cases}}
    \label{fig:cases}
  \end{figure}
\end{enumerate}
\end{document}

