\documentclass{article}
\usepackage{fullpage}
\usepackage{graphicx}
\usepackage{amsmath}
\usepackage[aux]{rerunfilecheck}

\newcommand{\ds}{\displaystyle}

\input{../common.tex}

\title{MATH 110 Midterm 1A Solutions}
\author{\commonAuthor}
\date{\commonDateMTOne}

\begin{document}
\maketitle
\begin{enumerate}
\item %1
  \begin{enumerate}
  \item We write $u(t) = t^{1/5} + 4(t^5)^{1/2} = t^{1/5} + 4t^{5/2}$
    so by the sum, constant multiple, and power rules we have
    $\ds u'(t) = \frac{1}{5} t^{1/5 - 1} + 4 \frac{5}{2} t^{5/2-1}
    = \frac{1}{5} t^{-4/5} + 10 t^{3/2}$.  Then
    $u'(1) = \frac{1}{5} t^{-4/5} + 10 1^{3/2} = 10.2$.
  \item By the quotient rule
    \begin{align*}
      y' = \frac{(1+r^{1/2})(r^2)' - r^2(1+r^{1/2})'}{(1+r^{1/2})^2}
      = \frac{(1+r^{1/2})2r - r^2((1/2)r^{-1/2})}{(1+r^{1/2})^2}
    \end{align*}
  \item By the quotient rule,
    \begin{align*}
      \frac{df}{dx} = \frac{(3-x)1'-1(3-x)'}{(3-x)^2} 
      = \frac{(3-x)0 -1(-1)}{(3-x)^2} 
      = \frac{1}{(3-x)^2}
      = \frac{1}{9-6x+x^2}
    \end{align*}
    Differentiating again,
    \begin{align*}
      \frac{d^2f}{dx^2}
      = \frac{(9-6x+x^2) 1'- 1(9-6x+x^2)'}{(9-6x+x^2)^2}
      = \frac{6-2x}{(9-6x+x^2)^2}
    \end{align*}
    Various simplifications are possible but are not necessary.
    However, if you want to check,
    you might want to simplify and compare with the second derivative of
    $(3-x)^{-1}$ calculated by the chain rule and the product rule.
  \end{enumerate}
\item Checking $x=7$ gives a result of $0/0$ so further work is necessary
  to evaluate the limit.  The usual strategy is to multiply top
  and bottom by the conjugate radical, i.e.,
  \begin{align*}
    \lim_{x\to 7} \frac{\sqrt{x+2}-3}{x-7}
    &= \lim_{x\to 7} \frac{\sqrt{x+2}-3}{x-7} \cdot 
    \frac{\sqrt{x+2}+3}{\sqrt{x+2}+3}
    \\
    &= \lim_{x\to 7} \frac{(x+2)-9}{(x-7)(\sqrt{x+2}+3)}
    \\
    &= \lim_{x\to 7} \frac{1}{\sqrt{x+2}+3}
    = \frac{1}{\sqrt{7+2}+3} = \frac{1}{6}
  \end{align*}
  because the function under the final limit above is continuous at $x=7$.
\item We can break this function into steps as follows:
  \begin{align*}
    f(a) &= \frac{3+a}{1-3a} \\
    f(a+h) &= \frac{3+(a+h)}{1-3(a+h)} \\
    f(a+h)-f(a) &= \frac{3+a+h}{1-3a-3h} - \frac{3+a}{1-3a}
    \\
    &= \frac{(3+a+h)(1-3a)-(1-3a-3h)(3+a)}{(1-3a-3h)(1-3a)}
    \\
    &= \frac{3+a+h-9a-3a^2-3ha - 3+9a+9h-a+3a^2+3ah}{(1-3a-3h)(1-3a)}
    \\
    &= \frac{10h}{(1-3a-3h)(1-3a)}
    \\
    f'(a) &= \lim_{h\to 0} \frac{f(a+h)-f(a)}{h}
    \\
    &= \lim_{h\to 0} \frac{10h}{(1-3a-3h)(1-3a)} \cdot \frac{1}{h}
    \\
    &= \lim_{h\to 0} \frac{10}{(1-3a-3h)(1-3a)}
    \\
    &= \frac{10}{(1-3a)^2}
  \end{align*}
  Avoid the urge to take bad shortcuts by cancelling incorrectly in the 
  fourth line of the calculation.

  You can check by differentiating using the quotient rule.
\item It is a good idea, but not necessary, to check that $y(1)=2$.  Now
  to get an equation of the tangent line we need a point on the line, which
  we have (namely $(1,2)$) and the slope of the line, which comes from
  the derivative.  By the quotient rule,
  \begin{align*}
    y' = \frac{(x^2+1)(3) - (3x+1)(2x)}{(x^2+1)^2}
  \end{align*}
  Algebraic simplifications are possible at this point
  but are counter-productive.  Substituting $x=1$ gives
  \begin{align*}
    y'(1) = \frac{(1^2+1)(3) - (3(1)+1)(2(1))}{(1^2+1)^2}
    = \frac{6-8}{2^2} = -\frac{1}{2}
  \end{align*}
  An equation of the tangent line is $\ds y-2=-\frac{1}{2} (x-1)$.
  The normal line passes through the same point $(1,2)$ but has negative
  reciprocal slope $m=2$, so the equation of the normal line is
  $y-2=2(x-1)$.

  Note that if you use the point-slope form of the equations of the lines
  instead of the slope-intercept form $y=mx+b$, you don't have to solve
  for $b$.
\item 
  \begin{enumerate}
  \item The function is continuous on $(-\infty,2)$ because it is given by
    the formula $cx^2+2x$ on that domain; similarly it is continuous on 
    $(2,\infty)$, so the only point in question is $x=2$.  The condition for
    continuity at that point is $\ds \lim_{x\to 2} f(x) = f(2)$.  We have
    \begin{align*}
      \lim_{x\to 2^-} f(x) &= \lim_{x\to 2^-} cx^2 + 2x = 4c+4 \\
      \lim_{x\to 2^+} f(x) &= \lim_{x\to 2^+} x^3 - cx = 8-2c \\
      f(2) &= 2^3-c(2) = 8-2c
    \end{align*}
    Note that we use the $x^3-cx$ definition when we evaluate $f(2)$ 
    because that definition applies on $2\le x < \infty$, an interval which
    includes $2$.
    For $\lim_{x\to 2} f(x)$ to exist, the above two limits must be equal, so
    $4c+4=8-2c$ which implies $6c=4$ or $c=2/3$, in which case the limit
    is $20/3$.  Since we also have $f(2)=20/3$ for that value of $c$, it follows
    that $f(x)$ is continuous if and only if $c=2/3$.
  \item A function can be differentiable only if it is continuous, so the
    only possible value of $c$ for $f(x)$ to be differentiable is $c=2/3$.
    When $c=2/3$ we have the left and right sided derivatives
    \begin{align*}
      \lim_{h\to 0^-} \frac{f(2+h)-f(2)}{h}
      &= \lim_{h\to 0^-} \frac{(8/3)+(8/3)h+(2/3)h^2+4+2h-20/3}{h}
      \\
      &= \lim_{h\to 0^-} \frac{(14/3)h + (2/3)h^2}{h} = \frac{14}{3}
      \\
      \lim_{h\to 0^+} \frac{f(2+h)-f(2)}{h}
      &= \lim_{h\to 0^+} \frac{8+12h+6h^2+h^3-(4/3)-(2/3)h-20/3}{h}
      \\
      &= \lim_{h\to 0^+} \frac{(32/3)h + 6h^2+h^3}{h} = \frac{32}{3}
    \end{align*}
    Since the left and right derivatives disagree at $x=2$ we have a corner
    point there and the function is not differentiable for $c=2/3$, so it
    is never differentiable.
  \end{enumerate}
\item Substituting $x=-2$ into the expression gives $\ds \frac{15-a}{0}$.
  That gives an infinite limit (which doesn't exist, of course) for all values
  of $a$ except possibly when $15-a=0$, 
  so the only possible value of $a$ which can give us a limit which exists
  is $a=15$.  Checking,
  \begin{align*}
    \lim_{x\to -2} \frac{3x^2+15x+18}{x^2+x-2}
    = \lim_{x\to -2} \frac{(3x+9)(x+2)}{(x+2)(x-1)}
    = \lim_{x\to -2} \frac{3x+9}{x-1}
    = \frac{3}{-3} = -1
  \end{align*}
  In conclusion, the limit exists if and only if $a=15$, in which case the
  limit is $-1$.
\end{enumerate}
\end{document}

